cleaning

yalla/ll_prop.v
@@ -8,6 +8,8 @@ From OLlibs Require Import dectype List_more
                            Dependent_Forall_Type flat_map_more.
 From Yalla Require Export ll_cut.
 
+Set Implicit Arguments.
+
 Section Atoms.
 
 Context {atom : DecType}.
@@ -16,7 +18,7 @@ Notation ll := (@ll atom).
 
 (** Consistency statements *)
 
-Lemma weak_consistency_axfree {P} : (projT1 (pgax P) -> False) -> pmix P 0 = false ->
+Lemma weak_consistency_axfree P : (projT1 (pgax P) -> False) -> pmix P 0 = false ->
   ll P nil -> False.
 Proof.
 intros Hgax Hmix0 pi.
@@ -38,25 +40,25 @@ remember nil as l; revert Heql; induction pi using ll_nested_ind; intros Heql; i
 - apply (Hgax a).
 Qed.
 
-Lemma strong_consistency_axfree {P} : (projT1 (pgax P) -> False) ->
- ll P (zero :: nil) -> False.
+Lemma strong_consistency_axfree P : (projT1 (pgax P) -> False) ->
+  ll P (zero :: nil) -> False.
 Proof.
 intros Hgax pi.
-apply cut_admissible_axfree in pi ; try assumption.
-remember (zero :: nil) as l ; revert Heql ; induction pi using ll_nested_ind ;
-  intros Heql ; inversion Heql ; subst.
+apply cut_admissible_axfree in pi; try assumption.
+remember (zero :: nil) as l; revert Heql; induction pi using ll_nested_ind;
+  intros Heql; inversion Heql; subst.
 - apply IHpi.
   symmetry in p.
   apply (PCPermutation_Type_length_1_inv _ _ _ p).
 - apply IHpi.
-  destruct l1 ; inversion Heql.
-  + destruct lw' ; inversion Heql.
-    symmetry in p ; apply Permutation_Type_nil in p ; subst.
-    destruct l2 ; inversion H ; subst ; reflexivity.
-  + apply app_eq_nil in H2 ; destruct H2 as [? H2] ; subst.
-    apply app_eq_nil in H2 ; destruct H2 as [H2 ?] ; subst.
-    destruct lw' ; inversion Heql.
-    symmetry in p ; apply Permutation_Type_nil in p ; subst ; reflexivity.
+  destruct l1; inversion Heql.
+  + destruct lw'; inversion Heql.
+    symmetry in p; apply Permutation_Type_nil in p; subst.
+    destruct l2; inversion_clear H; reflexivity.
+  + apply app_eq_nil in H2; destruct H2 as [? H2]; subst.
+    apply app_eq_nil in H2; destruct H2 as [H2 ?]; subst.
+    destruct lw'; inversion Heql.
+    symmetry in p; apply Permutation_Type_nil in p; subst; reflexivity.
 - revert PL X Heql; clear; induction L; intros PL HPL Heql; inversion Heql.
   inversion HPL as [ | ? ? ? ? Heq ]; destruct a; subst.
   + apply IHL with Fl; assumption.
@@ -69,43 +71,45 @@ Qed.
 
 
 (** Some additional reversibility statements *)
-Lemma with_rev1_noax {P} : (projT1 (pgax P) -> False) ->
-forall A B l1 l2, ll P (l1 ++ awith A B :: l2) -> ll P (l1 ++ A :: l2).
-Proof with myeeasy.
+(* TODO atomic gax should be enough *)
+
+Lemma with_rev1_noax P : (projT1 (pgax P) -> False) ->
+  forall A B l1 l2, ll P (l1 ++ awith A B :: l2) -> ll P (l1 ++ A :: l2).
+Proof.
 intros Hgax A B l1 l2 pi.
 assert (ll P (dual (awith A B) :: A :: nil)) as pi'.
 { apply plus_r1.
   eapply ex_r ; [ | apply PCPermutation_Type_swap ].
   apply ax_exp. }
 eapply (ex_r ((l2 ++ l1) ++ A :: nil)) ; [ | GPermutation_Type_solve ].
-eapply cut_r_axfree ; try eassumption.
-eapply ex_r ; [ apply pi | GPermutation_Type_solve ].
+eapply cut_r_axfree; try eassumption.
+eapply ex_r; [ apply pi | GPermutation_Type_solve ].
 Qed.
 
-Lemma with_rev2_noax {P} : (projT1 (pgax P) -> False) ->
-forall A B l1 l2, ll P (l1 ++ awith B A :: l2) -> ll P (l1 ++ A :: l2).
-Proof with myeeasy.
+Lemma with_rev2_noax P : (projT1 (pgax P) -> False) ->
+  forall A B l1 l2, ll P (l1 ++ awith B A :: l2) -> ll P (l1 ++ A :: l2).
+Proof.
 intros Hgax A B l1 l2 pi.
 assert (ll P (dual (awith B A) :: A :: nil)) as pi'.
 { apply plus_r2.
-  eapply ex_r ; [ | apply PCPermutation_Type_swap ].
+  eapply ex_r; [ | apply PCPermutation_Type_swap ].
   apply ax_exp. }
-eapply (ex_r ((l2 ++ l1) ++ A :: nil)) ; [ | GPermutation_Type_solve ].
-eapply cut_r_axfree ; try eassumption.
-eapply ex_r ; [ apply pi | GPermutation_Type_solve ].
+eapply (ex_r ((l2 ++ l1) ++ A :: nil)); [ | GPermutation_Type_solve ].
+eapply cut_r_axfree; try eassumption.
+eapply ex_r; [ apply pi | GPermutation_Type_solve ].
 Qed.
 
-Lemma oc_rev_noax {P} : (projT1 (pgax P) -> False) ->
+Lemma oc_rev_noax P : (projT1 (pgax P) -> False) ->
 forall A l1 l2, ll P (l1 ++ oc A :: l2) -> ll P (l1 ++ A :: l2).
-Proof with myeeasy.
+Proof.
 intros Hgax A l1 l2 pi.
 assert (ll P (dual (oc A) :: A :: nil)) as pi'.
 { apply de_r.
-  eapply ex_r ; [ | apply PCPermutation_Type_swap ].
+  eapply ex_r; [ | apply PCPermutation_Type_swap ].
   apply ax_exp. }
-eapply (ex_r ((l2 ++ l1) ++ A :: nil)) ; [ | GPermutation_Type_solve ].
-eapply cut_r_axfree ; try eassumption.
-eapply ex_r ; [ apply pi | GPermutation_Type_solve ].
+eapply (ex_r ((l2 ++ l1) ++ A :: nil)); [ | GPermutation_Type_solve ].
+eapply cut_r_axfree; try eassumption.
+eapply ex_r; [ apply pi | GPermutation_Type_solve ].
 Qed.
 
 
@@ -155,27 +159,27 @@ Section ll_ps_ind.
   Definition Forall_Proofs_ps (Pred : forall l, ll_ps P PS l -> Type) {L} (piL : Forall_inf (ll_ps P PS) L) :=
     Dependent_Forall_inf Pred piL.
 
-  Fixpoint ll_ps_nested_ind {l} (pi : ll_ps P PS l): forall (Pred : forall l, ll_ps P PS l -> Type),
+  Fixpoint ll_ps_nested_ind l (pi : ll_ps P PS l): forall (Pred : forall l, ll_ps P PS l -> Type),
     (forall X Hps, Pred (covar X :: var X :: nil) (ax_ps_r P PS X Hps)) ->
-    (forall l1 l2 Hps pi p, Pred l1 pi -> Pred l2 (ex_ps_r P PS l1 l2 Hps pi p)) ->
+    (forall l1 l2 Hps pi p, Pred l1 pi -> Pred l2 (ex_ps_r l2 Hps pi p)) ->
     (forall l1 lw lw' l2 Hps pi p, Pred (l1 ++ map wn lw ++ l2) pi ->
-      Pred (l1 ++ map wn lw' ++ l2) (ex_wn_ps_r P PS l1 lw lw' l2 Hps pi p)) ->
+      Pred (l1 ++ map wn lw' ++ l2) (ex_wn_ps_r l1 l2 Hps pi p)) ->
     (forall L eqpmix Hps PL, Forall_Proofs_ps Pred PL ->
-      Pred (concat L) (mix_ps_r P PS L eqpmix Hps PL)) ->
+      Pred (concat L) (mix_ps_r eqpmix Hps PL)) ->
     (forall Hps, Pred (one :: nil) (one_ps_r P PS Hps)) ->
-    (forall l Hps pi, Pred l pi -> Pred (bot :: l) (bot_ps_r P PS l Hps pi)) ->
+    (forall l Hps pi, Pred l pi -> Pred (bot :: l) (bot_ps_r Hps pi)) ->
     (forall A B l1 l2 Hps pi1 pi2, Pred (A :: l1) pi1 -> Pred (B :: l2) pi2 ->
-      Pred (tens A B :: l2 ++ l1) (tens_ps_r P PS A B l1 l2 Hps pi1 pi2)) ->
-    (forall A B l Hps pi, Pred (A :: B :: l) pi -> Pred (parr A B :: l) (parr_ps_r P PS A B l Hps pi)) ->
+      Pred (tens A B :: l2 ++ l1) (tens_ps_r Hps pi1 pi2)) ->
+    (forall A B l Hps pi, Pred (A :: B :: l) pi -> Pred (parr A B :: l) (parr_ps_r Hps pi)) ->
     (forall l Hps, Pred (top :: l) (top_ps_r P PS l Hps)) ->
-    (forall A B l Hps pi, Pred (A :: l) pi -> Pred (aplus A B :: l) (plus_ps_r1 P PS A B l Hps pi)) ->
-    (forall A B l Hps pi, Pred (A :: l) pi -> Pred (aplus B A :: l) (plus_ps_r2 P PS A B l Hps pi)) ->
+    (forall A B l Hps pi, Pred (A :: l) pi -> Pred (aplus A B :: l) (plus_ps_r1 B Hps pi)) ->
+    (forall A B l Hps pi, Pred (A :: l) pi -> Pred (aplus B A :: l) (plus_ps_r2 B Hps pi)) ->
     (forall A B l Hps pi1 pi2, Pred (A :: l) pi1 -> Pred (B :: l) pi2 ->
-      Pred (awith A B :: l) (with_ps_r P PS A B l Hps pi1 pi2)) ->
-    (forall A l Hps pi, Pred (A :: map wn l) pi -> Pred (oc A :: map wn l) (oc_ps_r P PS A l Hps pi)) ->
-    (forall A l Hps pi, Pred (A :: l) pi -> Pred (wn A :: l) (de_ps_r P PS A l Hps pi)) ->
-    (forall A l Hps pi, Pred l pi -> Pred (wn A :: l) (wk_ps_r P PS A l Hps pi)) ->
-    (forall A l Hps pi, Pred (wn A :: wn A :: l) pi -> Pred (wn A :: l) (co_ps_r P PS A l Hps pi)) ->
+      Pred (awith A B :: l) (with_ps_r Hps pi1 pi2)) ->
+    (forall A l Hps pi, Pred (A :: map wn l) pi -> Pred (oc A :: map wn l) (oc_ps_r l Hps pi)) ->
+    (forall A l Hps pi, Pred (A :: l) pi -> Pred (wn A :: l) (de_ps_r Hps pi)) ->
+    (forall A l Hps pi, Pred l pi -> Pred (wn A :: l) (wk_ps_r A Hps pi)) ->
+    (forall A l Hps pi, Pred (wn A :: wn A :: l) pi -> Pred (wn A :: l) (co_ps_r Hps pi)) ->
     (forall f A l1 l2 Hps pi1 pi2, Pred (dual A :: l1) pi1 -> Pred (A :: l2) pi2 ->
       Pred (l2 ++ l1) (@cut_ps_r P PS f A l1 l2 Hps pi1 pi2)) ->
     (forall a Hps, Pred (projT2 (pgax P) a) (gax_ps_r P PS a Hps)) ->
@@ -183,107 +187,101 @@ Section ll_ps_ind.
       fun Pred ax_case ex_case ex_wn_case mix_case one_case bot_case tens_case parr_case
                top_case plus_case1 plus_case2 with_case oc_case de_case wk_case co_case cut_case gax_case =>
     let rec_call {l} (pi : ll_ps P PS l) :=
-       (ll_ps_nested_ind pi Pred ax_case ex_case ex_wn_case mix_case one_case bot_case tens_case parr_case
-                                 top_case plus_case1 plus_case2 with_case
-                                 oc_case de_case wk_case co_case cut_case gax_case) in
+       (ll_ps_nested_ind pi ax_case ex_case ex_wn_case mix_case one_case bot_case tens_case parr_case
+                            top_case plus_case1 plus_case2 with_case
+                            oc_case de_case wk_case co_case cut_case gax_case) in
     match pi with
     | ax_ps_r _ _ X Hps => ax_case X Hps
-    | ex_ps_r _ _ l1 l2 Hps pi p => ex_case l1 l2 Hps pi p (rec_call pi)
-    | ex_wn_ps_r _ _ l1 lw lw' l2 Hps pi p => ex_wn_case l1 lw lw' l2 Hps pi p (rec_call pi)
-    | mix_ps_r _ _ L eqpmix Hps PL => mix_case L eqpmix Hps PL (
+    | @ex_ps_r _ _ l1 l2 Hps pi p => ex_case l1 l2 Hps pi p (rec_call pi)
+    | @ex_wn_ps_r _ _ l1 lw lw' l2 Hps pi p => ex_wn_case l1 lw lw' l2 Hps pi p (rec_call pi)
+    | @mix_ps_r _ _ L eqpmix Hps PL => mix_case L eqpmix Hps PL (
         (fix ll_ps_nested_ind_aux L (PL : Forall_inf (ll_ps P PS) L) : Forall_Proofs_ps Pred PL :=
           match PL with
           | Forall_inf_nil _ => Dependent_Forall_inf_nil _ Pred
           | @Forall_inf_cons _ _ l L Pil PiL => Dependent_Forall_inf_cons _ Pil (rec_call Pil)
                                                                             (ll_ps_nested_ind_aux L PiL)
           end) L PL)
-    | one_ps_r _ _ Hps => one_case Hps
-    | bot_ps_r _ _ l Hps pi => bot_case l Hps pi (rec_call pi)
-    | tens_ps_r _ _ A B l1 l2 Hps pi1 pi2 => tens_case A B l1 l2 Hps pi1 pi2 (rec_call pi1) (rec_call pi2)
-    | parr_ps_r _ _ A B l Hps pi => parr_case A B l Hps pi (rec_call pi)
-    | top_ps_r _ _ l Hps => top_case l Hps
-    | plus_ps_r1 _ _ A B l Hps pi => plus_case1 A B l Hps pi (rec_call pi)
-    | plus_ps_r2 _ _ A B l Hps pi => plus_case2 A B l Hps pi (rec_call pi)
-    | with_ps_r _ _ A B l Hps pi1 pi2 => with_case A B l Hps pi1 pi2 (rec_call pi1) (rec_call pi2)
-    | oc_ps_r _ _ A l Hps pi => oc_case A l Hps pi (rec_call pi)
-    | de_ps_r _ _ A l Hps pi => de_case A l Hps pi (rec_call pi)
-    | wk_ps_r _ _ A l Hps pi => wk_case A l Hps pi (rec_call pi)
-    | co_ps_r _ _ A l Hps pi => co_case A l Hps pi (rec_call pi)
+    | @one_ps_r _ _ Hps => one_case Hps
+    | @bot_ps_r _ _ l Hps pi => bot_case l Hps pi (rec_call pi)
+    | @tens_ps_r _ _ A B l1 l2 Hps pi1 pi2 => tens_case A B l1 l2 Hps pi1 pi2 (rec_call pi1) (rec_call pi2)
+    | @parr_ps_r _ _ A B l Hps pi => parr_case A B l Hps pi (rec_call pi)
+    | @top_ps_r _ _ l Hps => top_case l Hps
+    | @plus_ps_r1 _ _ A B l Hps pi => plus_case1 A B l Hps pi (rec_call pi)
+    | @plus_ps_r2 _ _ A B l Hps pi => plus_case2 A B l Hps pi (rec_call pi)
+    | @with_ps_r _ _ A B l Hps pi1 pi2 => with_case A B l Hps pi1 pi2 (rec_call pi1) (rec_call pi2)
+    | @oc_ps_r _ _ A l Hps pi => oc_case A l Hps pi (rec_call pi)
+    | @de_ps_r _ _ A l Hps pi => de_case A l Hps pi (rec_call pi)
+    | @wk_ps_r _ _ A l Hps pi => wk_case A l Hps pi (rec_call pi)
+    | @co_ps_r _ _ A l Hps pi => co_case A l Hps pi (rec_call pi)
     | @cut_ps_r _ _ f A l1 l2 Hps pi1 pi2 => cut_case f A l1 l2 Hps pi1 pi2 (rec_call pi1) (rec_call pi2)
     | gax_ps_r _ _ a Hps => gax_case a Hps
     end.
 
 End ll_ps_ind.
 
+Arguments ll_ps_nested_ind P PS {l}.
+
+
 Lemma stronger_ps_pfrag P Q : le_pfrag P Q -> forall PS l,
   ll_ps P PS l -> ll_ps Q PS l.
-Proof with myeeasy.
-intros Hle PS l H.
-induction H using (ll_ps_nested_ind P PS) ; try (econstructor ; myeeasy ; fail).
-- apply (ex_ps_r _ _ l1)...
+Proof.
+intros Hle PS l pi.
+induction pi using (ll_ps_nested_ind P PS); try (now constructor).
+- apply (@ex_ps_r _ _ l1); try assumption.
   destruct Hle as (_ & _ & _  & Hp).
-  unfold PCPermutation_Type in p.
-  unfold PCPermutation_Type.
-  destruct (pperm P) ; destruct (pperm Q) ;
-    cbn in Hp ; try inversion Hp...
-  apply CPermutation_Permutation_Type...
+  unfold PCPermutation_Type in *.
+  destruct (pperm P); destruct (pperm Q); cbn in Hp; try (inversion Hp; assumption).
+  apply CPermutation_Permutation_Type; assumption.
+- eapply ex_wn_ps_r; eassumption.
 - unfold le_pfrag in Hle.
   destruct Hle as (_ & _ & Hmix & _).
   specialize (Hmix (length L)).
-  rewrite eqpmix in Hmix.
-  cbn in Hmix...
-  apply mix_ps_r...
+  rewrite eqpmix in Hmix; cbn in Hmix.
+  apply mix_ps_r; try assumption.
   apply forall_Forall_inf.
   intros l' Hin.
   apply(In_Forall_inf_in _ PL) in Hin as [pi Hin].
   refine (Dependent_Forall_inf_forall_formula _ _ X Hin).
 - destruct Hle as [Hle _].
-  rewrite f in Hle.
-  cbn in Hle.
-  eapply (@cut_ps_r _ _ Hle)...
+  rewrite f in Hle; cbn in Hle.
+  apply (@cut_ps_r _ _ Hle A); assumption.
 - destruct Hle as (_ & Hgax & _).
   destruct (Hgax a) as [b Heq].
-  rewrite Heq in Hps ; rewrite Heq.
-  apply gax_ps_r...
+  rewrite Heq in Hps; rewrite Heq.
+  apply gax_ps_r; assumption.
 Qed.
 
-Lemma ll_ps_stronger {P} : forall PS QS l,
+Lemma ll_ps_stronger P PS QS l :
   ll_ps P PS l -> (forall x, is_true (PS x) -> is_true (QS x)) -> ll_ps P QS l.
-Proof with try eassumption.
-intros PS QS l pi Hs.
-induction pi using (ll_ps_nested_ind P PS) ; try (econstructor ; try apply Hs ; eassumption ; fail).
-apply mix_ps_r ; [ | apply Hs | ]...
-apply forall_Forall_inf.
-intros l' Hin.
-apply(In_Forall_inf_in _ PL) in Hin as [pi Hin].
-refine (Dependent_Forall_inf_forall_formula _ _ X Hin).
-Qed.
-
-Lemma ll_ps_is_ps {P} : forall l PS, ll_ps P PS l -> is_true (PS l).
 Proof.
-intros l PS Hll; inversion Hll; assumption.
-Qed.
-
-Lemma ll_ps_is_ll {P} : forall l PS, ll_ps P PS l -> ll P l.
-Proof with try eassumption.
-intros l PS pi.
-induction pi using (ll_ps_nested_ind P PS); try (econstructor ; eassumption ; fail).
-apply mix_r...
+intros pi Hs.
+induction pi using (ll_ps_nested_ind P PS); try now (econstructor; try apply Hs; eassumption).
+apply mix_ps_r ; [ | apply Hs | ]; try assumption.
 apply forall_Forall_inf.
 intros l' Hin.
 apply(In_Forall_inf_in _ PL) in Hin as [pi Hin].
-refine (Dependent_Forall_inf_forall_formula _ _ X Hin).
+apply (Dependent_Forall_inf_forall_formula _ _ X Hin).
 Qed.
 
-Lemma ll_is_ll_ps {P} : forall l, ll P l -> ll_ps P (fun _ => true) l.
-Proof with myeeasy.
-intros l pi.
-induction pi using ll_nested_ind ; try (econstructor ; myeeasy ; fail).
-apply mix_ps_r...
-apply forall_Forall_inf.
-intros l' Hin.
+Lemma ll_ps_is_ps P PS l : ll_ps P PS l -> is_true (PS l).
+Proof. intros Hll; inversion Hll; assumption. Qed.
+
+Lemma ll_ps_is_ll P PS l : ll_ps P PS l -> ll P l.
+Proof.
+intros pi; induction pi using (ll_ps_nested_ind P PS); try now (econstructor; eassumption).
+apply mix_r; [ assumption | ].
+apply forall_Forall_inf; intros l' Hin.
 apply(In_Forall_inf_in _ PL) in Hin as [pi Hin].
-refine (Dependent_Forall_inf_forall_formula _ _ X Hin).
+apply (Dependent_Forall_inf_forall_formula _ _ X Hin).
+Qed.
+
+Lemma ll_is_ll_ps P l : ll P l -> ll_ps P (fun _ => true) l.
+Proof.
+intros pi; induction pi using ll_nested_ind; try now (econstructor; try eassumption; reflexivity).
+apply mix_ps_r; try assumption; try reflexivity.
+apply forall_Forall_inf; intros l' Hin.
+apply(In_Forall_inf_in _ PL) in Hin as [pi Hin].
+apply (Dependent_Forall_inf_forall_formula _ _ X Hin).
 Qed.
 
 (** A fragment is a subset of formulas closed under subformula. *)
@@ -291,45 +289,43 @@ Definition fragment FS :=
   forall A : formula, is_true (FS A) -> forall B, subform B A -> is_true (FS B).
 
 (** Linear logic is conservative over its fragments (in the absence of cut). *)
-Lemma conservativity {P} : pcut P = false -> forall FS, fragment FS ->
+Lemma conservativity P : pcut P = false -> forall FS, fragment FS ->
   forall l, ll_ps P (fun _ => true) l -> is_true (forallb FS l) -> ll_ps P (forallb FS) l.
-Proof with try eassumption ; try reflexivity.
+Proof.
 intros P_cutfree FS HFS l pi.
-induction pi using (ll_ps_nested_ind P (fun _ => true)) ; intros HFrag.
-- apply ax_ps_r...
-- apply (ex_ps_r _ _ l1)...
+induction pi using (ll_ps_nested_ind P (fun _ => true)); intros HFrag.
+- apply ax_ps_r; assumption.
+- apply (@ex_ps_r _ _ l1); try assumption.
   apply IHpi.
   apply PCPermutation_Type_sym in p.
   unfold is_true in HFrag; rewrite forallb_forall in HFrag; apply Forall_forall in HFrag.
   apply forallb_forall, Forall_forall.
-  eapply PCPermutation_Type_Forall...
-- eapply ex_wn_ps_r...
+  eapply PCPermutation_Type_Forall; eassumption.
+- eapply ex_wn_ps_r; try eassumption.
   apply IHpi.
   unfold is_true in HFrag; rewrite forallb_forall in HFrag; apply Forall_forall in HFrag.
   apply forallb_forall, Forall_forall.
   apply (Permutation_Type_map wn) in p.
-  eapply Permutation_Type_Forall...
+  eapply Permutation_Type_Forall; try eassumption.
   GPermutation_Type_solve.
 - unfold is_true in HFrag; rewrite forallb_forall in HFrag; apply Forall_forall in HFrag.
-  apply mix_ps_r...
-  + apply forallb_forall, Forall_forall...
-  + apply forall_Forall_inf.
-    intros l' Hin.
+  apply mix_ps_r; [ assumption | | ].
+  + apply forallb_forall, Forall_forall; assumption.
+  + apply forall_Forall_inf; intros l' Hin.
     apply(In_Forall_inf_in _ PL) in Hin as [pi Hin].
     refine (Dependent_Forall_inf_forall_formula _ _ X Hin _).
     clear - Hin HFrag.
-    apply forallb_forall.
-    intros A Hin'.
-    apply (Forall_forall (fun x => is_true (FS x)) (concat L))...
+    apply forallb_forall; intros A Hin'.
+    apply (Forall_forall (fun x => is_true (FS x)) (concat L)); [ assumption | ].
     apply in_concat; exists l'.
     apply In_Forall_inf_to_In_inf in Hin.
-    apply in_inf_in in Hin; split...
-- apply one_ps_r...
-- apply bot_ps_r...
+    apply in_inf_in in Hin; split; assumption.
+- apply one_ps_r; assumption.
+- apply bot_ps_r; [ assumption | ].
   inversion HFrag.
   apply andb_true_iff in H0.
   destruct H0.
-  apply IHpi...
+  apply IHpi; assumption.
 - assert (HFrag2 := HFrag).
   cbn in HFrag.
   apply andb_true_iff in HFrag.
@@ -338,159 +334,153 @@ induction pi using (ll_ps_nested_ind P (fun _ => true)) ; intros HFrag.
   apply Forall_app in HFrag as [HFragl HFragr].
   rewrite Forall_forall, <- forallb_forall in HFragl.
   rewrite Forall_forall, <- forallb_forall in HFragr.
-  apply tens_ps_r...
-  + apply IHpi1...
-    cbn ; apply andb_true_iff ; split...
-    eapply HFS...
-    apply sub_tens_l...
-  + apply IHpi2...
-    cbn ; apply andb_true_iff ; split...
-    eapply HFS...
-    apply sub_tens_r...
+  apply tens_ps_r; [ assumption | | ].
+  + apply IHpi1.
+    cbn; apply andb_true_iff; split; [ | assumption ].
+    eapply HFS; [ eassumption | ].
+    apply sub_tens_l; reflexivity.
+  + apply IHpi2.
+    cbn; apply andb_true_iff; split; [ | assumption ].
+    eapply HFS; [ eassumption | ].
+    apply sub_tens_r; reflexivity.
 - inversion HFrag ; subst.
   apply andb_true_iff in H0 ; destruct H0.
-  apply parr_ps_r...
+  apply parr_ps_r; [ assumption | ].
   apply IHpi.
   cbn ; apply andb_true_iff ; split ;
-    [ | cbn ; apply andb_true_iff ; split ]...
-  + eapply HFS...
-    apply sub_parr_l...
-  + eapply HFS...
-    apply sub_parr_r...
-- apply top_ps_r...
-- inversion HFrag ; subst.
-  apply andb_true_iff in H0 ; destruct H0.
-  apply plus_ps_r1...
+    [ | cbn ; apply andb_true_iff ; split ]; [ | | assumption ].
+  + eapply HFS; [ eassumption | ].
+    apply sub_parr_l; reflexivity.
+  + eapply HFS; [ eassumption | ].
+    apply sub_parr_r; reflexivity.
+- apply top_ps_r; assumption.
+- inversion HFrag; subst.
+  apply andb_true_iff in H0; destruct H0.
+  apply plus_ps_r1; [ assumption | ];
   apply IHpi.
-  cbn ; apply andb_true_iff ; split...
-  eapply HFS...
-  apply sub_plus_l...
-- inversion HFrag ; subst.
-  apply andb_true_iff in H0 ; destruct H0.
-  apply plus_ps_r2...
+  cbn; apply andb_true_iff; split; [ | assumption ].
+  eapply HFS; [ eassumption | ].
+  apply sub_plus_l; reflexivity.
+- inversion HFrag; subst.
+  apply andb_true_iff in H0; destruct H0.
+  apply plus_ps_r2; [ assumption | ].
   apply IHpi.
-  cbn ; apply andb_true_iff ; split...
-  eapply HFS...
-  apply sub_plus_r...
-- inversion HFrag ; subst.
-  apply andb_true_iff in H0 ; destruct H0.
-  apply with_ps_r...
-  + apply IHpi1...
-    cbn ; apply andb_true_iff ; split...
-    eapply HFS...
-    apply sub_with_l...
-  + apply IHpi2...
-    cbn ; apply andb_true_iff ; split...
-    eapply HFS...
-    apply sub_with_r...
-- inversion HFrag ; subst.
-  apply andb_true_iff in H0 ; destruct H0.
-  apply oc_ps_r...
+  cbn; apply andb_true_iff; split; [ | assumption ].
+  eapply HFS; [ eassumption | ].
+  apply sub_plus_r; reflexivity.
+- inversion HFrag; subst.
+  apply andb_true_iff in H0; destruct H0.
+  apply with_ps_r; [ assumption | | ].
+  + apply IHpi1.
+    cbn; apply andb_true_iff; split; [ | assumption ].
+    eapply HFS; [ eassumption | ].
+    apply sub_with_l; reflexivity.
+  + apply IHpi2.
+    cbn; apply andb_true_iff; split; [ | assumption ].
+    eapply HFS; [ eassumption | ].
+    apply sub_with_r; reflexivity.
+- inversion HFrag; subst.
+  apply andb_true_iff in H0; destruct H0.
+  apply oc_ps_r; [ assumption | ].
   apply IHpi.
-  cbn ; apply andb_true_iff ; split...
-  eapply HFS...
-  apply sub_oc...
-- inversion HFrag ; subst.
-  apply andb_true_iff in H0 ; destruct H0.
-  apply de_ps_r...
+  cbn; apply andb_true_iff; split; [ | assumption ].
+  eapply HFS; [ eassumption | ].
+  apply sub_oc; reflexivity.
+- inversion HFrag; subst.
+  apply andb_true_iff in H0; destruct H0.
+  apply de_ps_r; [ assumption | ].
   apply IHpi.
-  cbn ; apply andb_true_iff ; split...
-  eapply HFS...
-  apply sub_wn...
-- inversion HFrag ; subst.
-  apply andb_true_iff in H0 ; destruct H0.
-  apply wk_ps_r...
-  apply IHpi...
-- inversion HFrag ; subst.
-  apply andb_true_iff in H0 ; destruct H0.
-  apply co_ps_r...
+  cbn ; apply andb_true_iff ; split; [ | assumption ].
+  eapply HFS; [ eassumption | ].
+  apply sub_wn; reflexivity.
+- inversion HFrag; subst.
+  apply andb_true_iff in H0; destruct H0.
+  apply wk_ps_r; [ assumption | ].
+  apply IHpi; assumption.
+- inversion HFrag; subst.
+  apply andb_true_iff in H0; destruct H0.
+  apply co_ps_r; [ assumption | ].
   apply IHpi.
-  cbn ; apply andb_true_iff ; split...
-- rewrite P_cutfree in f.
-  inversion f.
-- apply gax_ps_r...
+  cbn; apply andb_true_iff; split; assumption.
+- rewrite P_cutfree in f; inversion f.
+- apply gax_ps_r; assumption.
 Qed.
 
 (** Subformula property:
 any provable sequent is provable by a proof containing only subformulas of this sequent. *)
-Proposition subformula {P} : pcut P = false -> forall l,
+Proposition subformula P : pcut P = false -> forall l,
   ll P l -> ll_ps P (fun x => subformb_list x l) l.
-Proof with try eassumption ; try reflexivity.
+Proof.
 intros P_cutfree l pi.
 apply ll_is_ll_ps in pi.
-apply conservativity...
+apply conservativity; try assumption.
 - intros A Hf B Hs.
-  revert Hf ; clear - Hs ; induction l ; intro Hf ; inversion Hf ; subst.
-  cbn ; apply orb_true_iff.
+  revert Hf; clear - Hs; induction l; intro Hf; inversion Hf; subst.
+  cbn; apply orb_true_iff.
   apply orb_true_iff in H0.
   destruct H0.
-  + left; eapply subb_trans...
-    apply subb_sub...
-  + right; apply IHl...
+  + left; eapply subb_trans; [ | eassumption ].
+    apply subb_sub; assumption.
+  + right; apply IHl; assumption.
 - apply (subb_id_list l nil).
 Qed.
 
 (* Cut is admissible in any fragment with no axioms. *)
-Lemma cut_admissible_fragment_axfree {P} : (projT1 (pgax P) -> False) ->
+Lemma cut_admissible_fragment_axfree P : (projT1 (pgax P) -> False) ->
  forall FS, fragment FS -> forall l,
    ll_ps P (forallb FS) l -> ll_ps (cutrm_pfrag P) (forallb FS) l.
-Proof with myeeasy.
+Proof.
 intros P_axfree FS HFS l pi.
-apply conservativity...
+apply conservativity; trivial.
 - apply ll_is_ll_ps.
-  apply cut_admissible_axfree...
-  eapply ll_ps_is_ll...
-- destruct pi...
+  apply cut_admissible_axfree; [ assumption | ].
+  eapply ll_ps_is_ll; eassumption.
+- destruct pi; assumption.
 Qed.
 
 (** Linear logic (with no axioms) is conservative over its fragments. *)
-Lemma conservativity_axfree {P} : (projT1 (pgax P) -> False) ->
+Lemma conservativity_axfree P : (projT1 (pgax P) -> False) ->
   forall FS, fragment FS -> forall l,
     ll P l -> is_true (forallb FS l) -> ll_ps P (forallb FS) l.
-Proof with try eassumption ; try reflexivity.
+Proof.
 intros P_axfree FS Hf l pi HFS.
-apply cut_admissible_axfree in pi...
+apply cut_admissible_axfree in pi; [ | assumption ].
 apply ll_is_ll_ps in pi.
-eapply conservativity in pi...
-clear - pi ; induction pi using (ll_ps_nested_ind (cutrm_pfrag P) (forallb FS));
-  try (econstructor ; eassumption ; fail).
+eapply conservativity in pi; try eassumption; [ | reflexivity ].
+clear - pi; induction pi using (ll_ps_nested_ind (cutrm_pfrag P) (forallb FS));
+  try now (econstructor; eassumption).
 - cbn in eqpmix.
-  apply mix_ps_r...
-  apply forall_Forall_inf.
-  intros l' Hin.
+  apply mix_ps_r; [ assumption | assumption | ].
+  apply forall_Forall_inf; intros l' Hin.
   apply (In_Forall_inf_in _ PL) in Hin as [pi Hin].
-  refine (Dependent_Forall_inf_forall_formula _ _ X Hin).
-- eapply @cut_ps_r...
-  destruct P.
-  inversion f.
-- revert a Hps.
-  assert (pgax (cutrm_pfrag P) = pgax P) as Hcut by reflexivity.
-  rewrite Hcut.
-  apply gax_ps_r.
+  apply (Dependent_Forall_inf_forall_formula _ _ X Hin).
+- eapply @cut_ps_r; try eassumption.
+  destruct P; inversion f.
+- assert (pgax (cutrm_pfrag P) = pgax P) as Hcut by reflexivity.
+  revert a Hps; rewrite Hcut; apply gax_ps_r.
 Qed.
 
 
 (** ** Deduction Theorem *)
 
 (** Deduction lemma for linear logic. *)
-Lemma deduction_list {P} : pperm P = true -> pcut P = true -> forall lax l, 
-  ll (axupd_pfrag P (existT (fun x => x -> list formula) (sum _ { k | k < length lax })
+Lemma deduction_list P : pperm P = true -> pcut P = true -> forall lax l, 
+  ll (axupd_pfrag P (existT (fun x => x -> _) (sum _ { k | k < length lax })
                                 (fun a => match a with
                                           | inl x => projT2 (pgax P) x
                                           | inr x => nth (proj1_sig x) lax one :: nil
                                           end))) l
   -> ll P (l ++ map wn (map dual lax)).
-Proof with myeeasy.
+Proof.
 intros P_perm P_cut lax.
-induction lax ; intros l pi.
+induction lax; intros l pi.
 - list_simpl.
-  eapply stronger_pfrag...
-  nsplit 4...
-  cbn ; intros a.
-  destruct a.
-  + exists p...
-  + exfalso ; destruct s as [k Hlt] ; inversion Hlt.
-- remember (axupd_pfrag P (existT (fun x => x -> list formula) (sum _ { k | k < length lax })
+  eapply stronger_pfrag; [ | eassumption ].
+  repeat split; try reflexivity.
+  cbn; intros [a | [k Hlt]].
+  + exists a; reflexivity.
+  + exfalso; inversion Hlt.
+- remember (axupd_pfrag P (existT (fun x => x -> _) (sum _ { k | k < length lax })
                                   (fun a => match a with
                                             | inl x => projT2 (pgax P) x
                                             | inr x => nth (proj1_sig x) lax one :: nil
@@ -501,54 +491,54 @@ induction lax ; intros l pi.
   eapply ax_gen; [ | | | | refine (ext_wn (dual a :: nil) pi); assumption ];
     try (now rewrite HeqQ).
   cbn in pi; cbn; intros [p|s].
-  + eapply ex_r ; [ | apply PCPermutation_Type_cons_append ].
+  + eapply ex_r; [ | apply PCPermutation_Type_cons_append ].
     apply wk_r.
     assert ({ b | projT2 (pgax P) p = projT2 (pgax Q) b}) as [b Hgax]
-      by (subst ; cbn ; exists (inl p) ; reflexivity).
+      by (subst; cbn; exists (inl p); reflexivity).
     rewrite Hgax.
     apply gax_r.
   + destruct s as [k Hlen].
-    destruct k ; cbn.
-    * eapply ex_r ; [ | apply PCPermutation_Type_swap ].
+    destruct k; cbn.
+    * eapply ex_r; [ | apply PCPermutation_Type_swap ].
       apply de_r.
-      eapply ex_r ; [ | apply PCPermutation_Type_swap ].
+      eapply ex_r; [ | apply PCPermutation_Type_swap ].
       apply ax_exp.
-    * eapply ex_r ; [ | apply PCPermutation_Type_swap ].
+    * eapply ex_r; [ | apply PCPermutation_Type_swap ].
       apply wk_r.
       assert ({ b | nth k lax one :: nil = projT2 (pgax Q) b}) as [b Hgax].
-      { subst ; cbn ; clear - Hlen.
+      { subst; cbn; clear - Hlen.
         apply PeanoNat.Nat.succ_lt_mono in Hlen.
-        exists (inr (exist _ k Hlen))... }
+        exists (inr (exist _ k Hlen)); reflexivity. }
       rewrite Hgax.
       apply gax_r.
 Qed.
 
 Lemma deduction_list_inv {P} : pperm P = true -> pcut P = true -> forall lax l, 
   ll P (l ++ map wn (map dual lax)) ->
-  ll (axupd_pfrag P (existT (fun x => x -> list formula) (sum _ { k | k < length lax })
+  ll (axupd_pfrag P (existT (fun x => x -> _) (sum _ { k | k < length lax })
                                 (fun a => match a with
                                           | inl x => projT2 (pgax P) x
                                           | inr x => nth (proj1_sig x) lax one :: nil
                                           end))) l.
-Proof with myeeasy.
+Proof.
 intros P_perm P_cut lax.
-induction lax ; intros l pi.
+induction lax; intros l pi.
 - list_simpl in pi.
-  eapply stronger_pfrag...
-  nsplit 4...
-  cbn ; intros a.
-  exists (inl a)...
+  eapply stronger_pfrag; [ | eassumption ].
+  repeat split; try reflexivity.
+  cbn; intros a.
+  exists (inl a); reflexivity.
 - list_simpl in pi.
   cons2app in pi.
   rewrite app_assoc in pi.
   apply IHlax in pi.
   rewrite <- (app_nil_r l).
-  refine (cut_r (wn (dual a)) _ _)...
-  + cbn ; rewrite bidual.
+  refine (cut_r (wn (dual a)) _ _); [ assumption | | ].
+  + cbn; rewrite bidual.
     change nil with (map (@wn atom) nil).
-    apply oc_r ; cbn.
+    apply oc_r; cbn.
     assert ({ b | a :: nil = projT2 (pgax (axupd_pfrag P
-     (existT (fun x => x -> list formula) (sum _ {k | k < S (length lax)})
+     (existT (fun x => x -> _) (sum _ {k | k < S (length lax)})
         (fun a0 => match a0 with
                    | inl x => projT2 (pgax P) x
                    | inr x => match proj1_sig x with
@@ -556,52 +546,48 @@ induction lax ; intros l pi.
                               | S m => nth m lax one
                               end :: nil
                    end)))) b}) as [b Hgax]
-      by (clear ; cbn ; exists (inr (exist _ 0 (le_n_S _ _ (le_0_n _)))) ; reflexivity).
+      by (clear; cbn; exists (inr (exist _ 0 (le_n_S _ _ (le_0_n _)))); reflexivity).
     rewrite Hgax.
     apply gax_r.
-  + eapply ex_r ; [ | apply PCPermutation_Type_sym ; apply PCPermutation_Type_cons_append ].
-    eapply stronger_pfrag...
-    nsplit 4...
-    cbn ; intros a'.
-    destruct a'.
-    * exists (inl p)...
-    * destruct s as [k Hlen] ; cbn.
-      apply PeanoNat.Nat.succ_lt_mono in Hlen.
-      exists (inr (exist _ (S k) Hlen))...
+  + eapply ex_r; [ | apply PCPermutation_Type_sym, PCPermutation_Type_cons_append ].
+    eapply stronger_pfrag; [ | eassumption ].
+    repeat split; try reflexivity.
+    cbn; intros [p | [k Hlen] ].
+    * exists (inl p); reflexivity.
+    * cbn.
+      apply -> PeanoNat.Nat.succ_lt_mono in Hlen.
+      exists (inr (exist _ (S k) Hlen)); reflexivity.
 Qed.
 
-Lemma deduction {P} : pperm P = true -> (projT1 (pgax P) -> False) -> pcut P = true -> forall lax l,
+Lemma deduction P : pperm P = true -> (projT1 (pgax P) -> False) -> pcut P = true -> forall lax l,
   ll (axupd_pfrag P (existT (fun x => x -> list formula) { k | k < length lax }
                             (fun a => nth (proj1_sig a) lax one :: nil))) l
     -> ll (cutrm_pfrag P) (l ++ (map wn (map dual lax))).
-Proof with myeeasy.
-intros P_perm P_axfree P_cut lax l ; intros pi.
-apply cut_admissible_axfree...
-apply deduction_list...
-eapply stronger_pfrag...
-nsplit 4...
-cbn ; intros a.
-exists (inr a)...
+Proof.
+intros P_perm P_axfree P_cut lax l pi.
+apply cut_admissible_axfree; [ assumption | ].
+apply deduction_list; [ assumption | assumption | ].
+eapply stronger_pfrag; [ | eassumption ].
+repeat split; try reflexivity.
+intros a; exists (inr a); reflexivity.
 Qed.
 
-Lemma deduction_inv {P} : pperm P = true -> (projT1 (pgax P) -> False) -> pcut P = true -> forall lax l,
+Lemma deduction_inv P : pperm P = true -> (projT1 (pgax P) -> False) -> pcut P = true -> forall lax l,
   ll (cutrm_pfrag P) (l ++ (map wn (map dual lax))) ->
   ll (axupd_pfrag P (existT (fun x => x -> list formula) { k | k < length lax }
                             (fun a => nth (proj1_sig a) lax one :: nil))) l.
-Proof with myeeasy.
-intros P_perm P_axfree P_cut lax l ; intros pi.
+Proof.
+intros P_perm P_axfree P_cut lax l pi.
 assert (ll P (l ++ (map wn (map dual lax)))) as pi'.
-{ eapply stronger_pfrag...
-  nsplit 4...
-  cbn ; intros a.
-  exists a... }
-apply deduction_list_inv in pi'...
-eapply stronger_pfrag...
-nsplit 4...
-cbn ; intros a.
-destruct a.
+{ eapply stronger_pfrag; [ | eassumption ].
+  repeat split; try reflexivity.
+  intros a; exists a; reflexivity. }
+apply deduction_list_inv in pi'; [ | assumption | assumption ].
+eapply stronger_pfrag; [ | eassumption ].
+repeat split; try reflexivity.
+cbn; intros a; destruct a as [? | s].
 - contradiction P_axfree.
-- exists s...
+- exists s; reflexivity.
 Qed.
 
 End Atoms.
