yalla/bbb.v
@@ -8,6 +8,7 @@ From OLlibs Require Import infinite List_more
                            Permutation_Type_more Permutation_Type_solve Dependent_Forall_Type.
 From Yalla Require Import ll_fragments.
 
+Set Implicit Arguments.
 
 Section Atoms.
 
@@ -38,186 +39,174 @@ Inductive ll_bbb : list formula -> Type :=
 | co_bbb_r : forall A l, ll_bbb (wn A :: wn A :: l) -> ll_bbb (wn A :: l).
 
 (** Generalized weakening for lists *)
-Lemma wk_list_bbb_r : forall l l', ll_bbb l' ->
-  ll_bbb (map wn l ++ l').
-Proof with myeeasy.
-induction l ; intros...
-apply wk_bbb_r.
-apply IHl...
+Lemma wk_list_bbb_r l l' : ll_bbb l' -> ll_bbb (map wn l ++ l').
+Proof.
+induction l; intros; [ assumption | ].
+cbn; apply wk_bbb_r.
+apply IHl; assumption.
 Qed.
 
 (** Generalized contraction for lists *)
-Lemma co_list_bbb_r : forall l l',
-ll_bbb (map wn l ++ map wn l ++ l') -> ll_bbb (map wn l ++ l').
-Proof with myeeasy.
-induction l ; intros...
-apply (ex_bbb_r (map wn l ++ wn a :: l')); [ | Permutation_Type_solve ].
+Lemma co_list_bbb_r l l' :
+  ll_bbb (map wn l ++ map wn l ++ l') -> ll_bbb (map wn l ++ l').
+Proof.
+induction l in l' |- *; intros; [ assumption | ].
+apply (@ex_bbb_r (map wn l ++ wn a :: l')); [ | Permutation_Type_solve ].
 apply IHl.
-apply (ex_bbb_r (wn a :: map wn l ++ map wn l ++ l')); [ | Permutation_Type_solve ].
+apply (@ex_bbb_r (wn a :: map wn l ++ map wn l ++ l')); [ | Permutation_Type_solve ].
 apply co_bbb_r.
-eapply ex_bbb_r; [ apply X | Permutation_Type_solve ].
+eapply ex_bbb_r; [ eassumption | Permutation_Type_solve ].
 Qed.
 
 (** Reversibility of [bot] in [ll_bbb] *)
-Lemma bot_rev_bbb : forall l, ll_bbb l ->
+Lemma bot_rev_bbb l : ll_bbb l ->
   forall l1 l2, l = l1 ++ bot :: l2 -> ll_bbb (l1 ++ l2).
-Proof with myeeasy.
-intros l pi; induction pi; intros l1' l2' Heq; subst.
+Proof.
+intros pi; induction pi; intros l1' l2' Heq; subst.
 - exfalso.
-  destruct l1' ; inversion Heq.
-  destruct l1' ; inversion H1.
-  destruct l1' ; inversion H3.
+  destruct l1'; inversion Heq.
+  destruct l1'; inversion H1.
+  destruct l1'; inversion H3.
 - assert (HP := p).
   apply Permutation_Type_vs_elt_inv in p.
-  destruct p as [(l3 & l4) Heq] ; cbn in Heq ; subst.
+  destruct p as [(l3 & l4) Heq]; cbn in Heq; subst.
   apply Permutation_Type_app_inv in HP.
-  eapply ex_bbb_r ; [ | apply HP ].
-  apply IHpi...
-- dichot_elt_app_inf_exec Heq ; subst.
-  + rewrite app_assoc ; apply mix2_bbb_r...
-    eapply bot_rev...
-    intros a ; destruct a.
-  + rewrite <- app_assoc ; apply mix2_bbb_r...
-    apply IHpi...
+  eapply ex_bbb_r; [ | apply HP ].
+  apply IHpi; reflexivity.
+- dichot_elt_app_inf_exec Heq; subst.
+  + rewrite app_assoc; apply mix2_bbb_r; [ assumption | ].
+    apply bot_rev; [ | assumption ].
+    intros a; destruct a.
+  + rewrite <- app_assoc; apply mix2_bbb_r; [ | assumption ].
+    apply IHpi; reflexivity.
 - exfalso.
-  destruct l1' ; inversion Heq.
-  destruct l1' ; inversion H1.
-- destruct l1' ; inversion Heq ; subst...
-  list_simpl ; eapply bot_bbb_r.
-  apply IHpi...
-- rewrite app_comm_cons in Heq ; dichot_elt_app_inf_exec Heq ; subst.
-  + destruct l1' ; inversion Heq0 ; subst.
+  destruct l1'; inversion Heq.
+  destruct l1'; inversion H1.
+- destruct l1'; inversion Heq ; subst; [ assumption | ].
+  list_simpl; apply bot_bbb_r.
+  apply IHpi; reflexivity.
+- rewrite app_comm_cons in Heq; dichot_elt_app_inf_exec Heq; subst.
+  + destruct l1'; inversion Heq0; subst.
     list_simpl.
-    rewrite app_assoc ; apply tens_bbb_r...
-    rewrite app_comm_cons.
-    apply IHpi2...
+    rewrite app_assoc; apply tens_bbb_r; [ assumption | ].
+    rewrite app_comm_cons; apply IHpi2; reflexivity.
   + list_simpl.
-    apply tens_bbb_r...
-    rewrite app_comm_cons.
-    apply IHpi1...
-- destruct l1' ; inversion Heq ; subst.
+    apply tens_bbb_r; [ | assumption ].
+    rewrite app_comm_cons; apply IHpi1; reflexivity.
+- destruct l1'; inversion Heq; subst.
   rewrite 2 app_comm_cons in IHpi.
-  list_simpl ; eapply parr_bbb_r...
-  rewrite 2 app_comm_cons.
-  apply IHpi...
-- destruct l1' ; inversion Heq ; subst.
-  list_simpl ; apply top_bbb_r...
-- destruct l1' ; inversion Heq ; subst.
-  list_simpl ; eapply plus_bbb_r1...
-  rewrite app_comm_cons.
-  apply IHpi...
-- destruct l1' ; inversion Heq ; subst.
-  list_simpl ; eapply plus_bbb_r2...
-  rewrite app_comm_cons.
-  apply IHpi...
-- destruct l1' ; inversion Heq ; subst.
-  list_simpl ; eapply with_bbb_r...
-  + rewrite app_comm_cons.
-    apply IHpi1...
-  + rewrite app_comm_cons.
-    apply IHpi2...
+  list_simpl; apply parr_bbb_r.
+  rewrite 2 app_comm_cons; apply IHpi; reflexivity.
+- destruct l1'; inversion Heq; subst.
+  list_simpl; apply top_bbb_r.
+- destruct l1'; inversion Heq; subst.
+  list_simpl; apply plus_bbb_r1.
+  rewrite app_comm_cons; apply IHpi; reflexivity.
+- destruct l1'; inversion Heq; subst.
+  list_simpl; apply plus_bbb_r2.
+  rewrite app_comm_cons; apply IHpi; reflexivity.
+- destruct l1'; inversion Heq; subst.
+  list_simpl; apply with_bbb_r.
+  + rewrite app_comm_cons; apply IHpi1; reflexivity.
+  + rewrite app_comm_cons; apply IHpi2; reflexivity.
 - exfalso.
-  destruct l1' ; inversion Heq.
+  destruct l1'; inversion Heq.
   decomp_map H1; inversion H1.
-- destruct l1' ; inversion Heq ; subst.
-  list_simpl ; eapply de_bbb_r...
-  rewrite app_comm_cons.
-  apply IHpi...
-- destruct l1' ; inversion Heq ; subst.
-  list_simpl ; eapply wk_bbb_r...
-  apply IHpi...
-- destruct l1' ; inversion Heq ; subst.
-  list_simpl ; eapply co_bbb_r...
-  rewrite 2 app_comm_cons.
-  apply IHpi...
+- destruct l1'; inversion Heq; subst.
+  list_simpl; apply de_bbb_r.
+  rewrite app_comm_cons; apply IHpi; reflexivity.
+- destruct l1'; inversion Heq; subst.
+  list_simpl; apply wk_bbb_r.
+  apply IHpi; reflexivity.
+- destruct l1'; inversion Heq; subst.
+  list_simpl; apply co_bbb_r.
+  rewrite 2 app_comm_cons; apply IHpi; reflexivity.
 Qed.
 
 (** [ll_mix2] is contained in [ll_bbb] *)
-Lemma mix2_to_bbb : forall l, ll_mix2 l -> ll_bbb l.
-Proof with myeeasy.
-intros l H ; induction H using ll_nested_ind ; try now constructor.
-- apply (ex_bbb_r l1)...
+Lemma mix2_to_bbb l : ll_mix2 l -> ll_bbb l.
+Proof.
+intros pi; induction pi using ll_nested_ind; try now constructor.
+- apply (@ex_bbb_r l1); assumption.
 - apply (Permutation_Type_map wn) in p.
-  eapply ex_bbb_r...
+  eapply ex_bbb_r; [ eassumption | ].
   Permutation_Type_solve.
 - repeat (destruct L; try now inversion eqpmix).
   cbn; rewrite app_nil_r.
   assert (ll_bbb l0) as pi1.
   { destruct (In_Forall_inf_in _ PL (in_inf_elt l0 (l :: nil) nil)) as [pi Hin].
-    refine (Dependent_Forall_inf_forall_formula _ _ X Hin). }
+    apply (Dependent_Forall_inf_forall_formula _ _ X Hin). }
   inversion PL; inversion X1; subst; clear X1 X2 X3.
-  apply mix2_bbb_r...
-  eapply stronger_pfrag...
-  nsplit 4...
-  + intros a ; exists a...
+  apply mix2_bbb_r; [ assumption | ].
+  eapply stronger_pfrag; [ | eassumption ].
+  repeat split.
+  + intros a; exists a; reflexivity.
   + intro n.
     repeat (destruct n; try apply BoolOrder.le_refl; try apply BoolOrder.le_true).
 - destruct a.
 Qed.
 
 (** [ll_bbb] is contained in [ll_mix02] *)
-Lemma bbb_to_mix02 : forall l, ll_bbb l -> ll_mix02 l.
-Proof with myeasy.
-intros l H ; induction H ; try now constructor.
-- apply (ex_r l1)...
+Lemma bbb_to_mix02 l : ll_bbb l -> ll_mix02 l.
+Proof.
+intros pi; induction pi; try now constructor.
+- apply (ex_r l1); assumption.
 - rewrite <- (app_nil_r _), <- app_assoc.
   change (l2 ++ l1 ++ nil) with (concat (l2 :: l1 :: nil)).
-  apply mix_r...
-  do 2 (apply Forall_inf_cons; try assumption).
-  apply Forall_inf_nil.
+  apply mix_r; [ reflexivity | ].
+  repeat constructor; assumption.
 Qed.
 
-Lemma mix2_std_bbb_r : forall l1 l2,
-  ll_bbb l1 -> ll_bbb l2 -> ll_bbb (l2 ++ l1).
+Lemma mix2_std_bbb_r l1 l2 : ll_bbb l1 -> ll_bbb l2 -> ll_bbb (l2 ++ l1).
 Proof.
-intros l1 l2 pi1 pi2.
-apply bbb_to_mix02 in pi2.
-apply mix2_bbb_r ; assumption.
+intros pi1 pi2%bbb_to_mix02.
+apply mix2_bbb_r; assumption.
 Qed.
 
 (** [ll_bbb] as an enriched [ll] system *)
 
-Lemma bbb_to_ll : forall l,
-  ll_bbb l -> ll_ll (wn (tens (wn one) bot) :: l).
-Proof with myeeasy ; try (cbn; Permutation_Type_solve).
-intros l pi; induction pi;
+Lemma bbb_to_ll l : ll_bbb l -> ll_ll (wn (tens (wn one) bot) :: l).
+Proof.
+intros pi; induction pi;
   (try now (apply wk_r ; constructor)) ;
   try now (eapply ex_r ; [ | apply Permutation_Type_swap ] ;
            constructor ; eapply ex_r ; [ eassumption | cbn; Permutation_Type_solve ]).
-- eapply ex_r...
-- apply co_r.
-  apply co_r.
-  apply de_r.
+- eapply ex_r; [ eassumption | cbn; Permutation_Type_solve ].
+- apply co_r, co_r, de_r.
   apply (ex_r (tens (wn one) bot :: (wn (tens (wn one) bot) :: l1)
-                                 ++ (wn (tens (wn one) bot) :: l2)))...
-  apply tens_r...
-  + apply mix02_to_ll'' with true true true...
-    apply stronger_pfrag with (pfrag_mix02)...
-    nsplit 4...
-    * intro a; split with a...
+                                 ++ (wn (tens (wn one) bot) :: l2)));
+    [ | cbn; Permutation_Type_solve ].
+  apply tens_r.
+  + apply mix02_to_ll'' with true true true; [ reflexivity | ].
+    apply stronger_pfrag with (pfrag_mix02); [ | assumption ].
+    repeat split.
+    * intro a; split with a; reflexivity.
     * intros n.
       repeat (destruct n; try reflexivity).
-  + apply bot_r...
+  + apply bot_r; assumption.
 - apply co_r.
   apply (ex_r (tens A B :: (wn (tens (wn one) bot) :: l2)
-                        ++ (wn (tens (wn one) bot) :: l1)))...
-  apply tens_r ; eapply ex_r ; [ apply IHpi1 | | apply IHpi2 | ] ...
-- eapply ex_r ; [ | apply Permutation_Type_swap ].
+                        ++ (wn (tens (wn one) bot) :: l1)));
+    [ | cbn; Permutation_Type_solve ].
+  apply tens_r; eapply ex_r; [ apply IHpi1 | | apply IHpi2 | ];
+    cbn; Permutation_Type_solve.
+- eapply ex_r; [ | apply Permutation_Type_swap ].
   apply with_r.
-  + eapply ex_r ; [ apply IHpi1 | ]...
-  + eapply ex_r ; [ apply IHpi2 | ]...
-- apply (ex_r (oc A :: map wn (tens (wn one) bot :: l)))...
+  + eapply ex_r; [ apply IHpi1 | cbn; Permutation_Type_solve ].
+  + eapply ex_r; [ apply IHpi2 | cbn; Permutation_Type_solve ].
+- apply (ex_r (oc A :: map wn (tens (wn one) bot :: l)));
+    [ | cbn; Permutation_Type_solve ].
   apply oc_r.
-  eapply ex_r...
+  eapply ex_r; [ eassumption | cbn; Permutation_Type_solve ].
 Qed.
 
-Lemma ll_to_bbb : forall l,
-  ll_ll l -> forall l' (l0 l1 : list unit),
-  Permutation_Type l (l' ++ map (fun _ => tens (wn one) bot) l1
-                         ++ map (fun _ => wn (tens (wn one) bot)) l0)  ->
+Lemma ll_to_bbb l : ll_ll l ->
+  forall l' (l0 l1 : list unit),
+    Permutation_Type l (l' ++ map (fun _ => tens (wn one) bot) l1
+                           ++ map (fun _ => wn (tens (wn one) bot)) l0)  ->
   ll_bbb l'.
-Proof with myeeasy ; try (cbn; Permutation_Type_solve).
-intros l pi; induction pi using ll_nested_ind; intros l' l0' l1' HP.
+Proof.
+intros pi; induction pi using ll_nested_ind; intros l' l0' l1' HP.
 - assert (HP' := HP).
   symmetry in HP'.
   apply Permutation_Type_vs_cons_inv in HP'.
@@ -227,34 +216,34 @@ intros l pi; induction pi using ll_nested_ind; intros l' l0' l1' HP.
   apply Permutation_Type_length_1_inv in HP.
   apply app_eq_unit_inf in HP.
   destruct HP as [[Heq1 Heq2] | [Heq1 Heq2]] ; subst ; destruct l' ; inversion Heq ; subst.
-  + destruct l1' ; inversion H0.
-    destruct l0' ; inversion H1.
-  + destruct l' ; inversion H1.
-    * destruct l1' ; inversion H0.
-      destruct l0' ; inversion H2.
-    * destruct l' ; inversion H2.
+  + destruct l1'; inversion H0.
+    destruct l0'; inversion H1.
+  + destruct l'; inversion H1.
+    * destruct l1'; inversion H0.
+      destruct l0'; inversion H2.
+    * destruct l'; inversion H2.
       rewrite H3.
       apply ax_bbb_r.
-  + destruct l1' ; inversion H0.
-    destruct l0' ; inversion H1.
-  + destruct l' ; inversion H1.
-    * destruct l1' ; inversion H0.
-      destruct l0' ; inversion H2.
-    * destruct l' ; inversion H2.
+  + destruct l1'; inversion H0.
+    destruct l0'; inversion H1.
+  + destruct l'; inversion H1.
+    * destruct l1'; inversion H0.
+      destruct l0'; inversion H2.
+    * destruct l'; inversion H2.
       rewrite H3.
-      eapply ex_bbb_r ; [ apply ax_bbb_r | ]...
+      eapply ex_bbb_r ; [ apply ax_bbb_r | apply Permutation_Type_swap ].
 - cbn in p.
   eapply IHpi.
-  etransitivity...
+  transitivity l2; eassumption.
 - eapply IHpi.
-  etransitivity...
-  apply (Permutation_Type_map wn) in p ; Permutation_Type_solve.
+  etransitivity; [ | eassumption ].
+  apply (Permutation_Type_map wn) in p; Permutation_Type_solve.
 - inversion eqpmix.
 - apply Permutation_Type_length_1_inv in HP.
-  destruct l' ; inversion HP.
-  + destruct l1' ; inversion H0.
-    destruct l0' ; inversion H1.
-  + apply app_eq_nil in H1 ; destruct H1 ; subst.
+  destruct l'; inversion HP.
+  + destruct l1'; inversion H0.
+    destruct l0'; inversion H1.
+  + apply app_eq_nil in H1; destruct H1; subst.
     apply one_bbb_r.
 - assert (HP' := HP).
   symmetry in HP'.
@@ -265,8 +254,8 @@ intros l pi; induction pi using ll_nested_ind; intros l' l0' l1' HP.
   dichot_elt_app_inf_exec Heq ; subst.
   + rewrite app_assoc in HP.
     apply IHpi in HP.
-    eapply ex_bbb_r ; [ apply bot_bbb_r | ]...
-  + dichot_elt_app_inf_exec Heq1 ; subst.
+    eapply ex_bbb_r; [ apply bot_bbb_r; eassumption | apply Permutation_Type_cons_app; reflexivity ].
+  + dichot_elt_app_inf_exec Heq1; subst.
     * symmetry in Heq0; decomp_map_inf Heq0; inversion Heq0.
     * symmetry in Heq2; decomp_map_inf Heq2; inversion Heq2.
 - assert (HP' := HP).
@@ -275,7 +264,7 @@ intros l pi; induction pi using ll_nested_ind; intros l' l0' l1' HP.
   destruct HP' as [[l'l l'r] Heq] ; cbn in Heq.
   rewrite Heq in HP.
   apply Permutation_Type_cons_app_inv in HP.
-  dichot_elt_app_inf_exec Heq ; subst.
+  dichot_elt_app_inf_exec Heq; subst.
   + rewrite app_assoc in HP.
     remember (l'l ++ l) as l'.
     apply Permutation_Type_app_app_inv in HP as [[[[l1a l2a] l3a] l4a] [[HP1 HP2] [HP3 HP4]]];
@@ -300,12 +289,12 @@ intros l pi; induction pi using ll_nested_ind; intros l' l0' l1' HP.
     apply IHpi2 in IHP2.
     symmetry in HP3.
     apply (Permutation_Type_cons_app _ _ (tens A B)) in HP3.
-    eapply ex_bbb_r ; [ apply tens_bbb_r | apply HP3 ]...
-  + dichot_elt_app_inf_exec Heq1 ; subst.
+    eapply ex_bbb_r ; [ apply tens_bbb_r | apply HP3 ]; assumption.
+  + dichot_elt_app_inf_exec Heq1; subst.
     * symmetry in Heq0; decomp_map_inf Heq0; inversion Heq0; subst; list_simpl in HP.
       rewrite (app_assoc (map _ l4)) in HP.
       rewrite <- map_app in HP.
-      remember (l4 ++ l6) as l0 ; clear Heql0.
+      remember (l4 ++ l6) as l0; clear Heql0.
       apply Permutation_Type_app_app_inv in HP as [[[[l1a l2a] l3a] l4a] [[HP1 HP2] [HP3 HP4]]];
         cbn in HP1, HP2, HP3, HP4.
       apply Permutation_Type_app_app_inv in HP4 as [[[[l1b l2b] l3b] l4b] [[HP1b HP2b] [HP3b HP4b]]];
@@ -320,103 +309,105 @@ intros l pi; induction pi using ll_nested_ind; intros l' l0' l1' HP.
       assert (IHP1 := Permutation_Type_trans HP2 HP4b).
       eapply (ex_r _ ((l2a ++ map (fun _ : unit => tens (wn one) bot) l7)
                        ++ map (fun _ => wn one) (tt :: nil)
-                       ++ map (fun _ => wn (tens (wn one) bot)) l9)) in pi1...
+                       ++ map (fun _ => wn (tens (wn one) bot)) l9)) in pi1;
+        [ | cbn; Permutation_Type_solve ].
       assert (ll pfrag_ll (l2a ++ wn one ::
                    map (fun _ : unit => wn (tens (wn one) bot)) (l7 ++ l9)))
         as pi1'.
       { clear - pi1; revert l2a l9 pi1; induction l7; intros l1 l2 pi;
-          list_simpl in pi; list_simpl...
+          list_simpl in pi; list_simpl; [ assumption | ].
         list_simpl in IHl7.
         apply (ex_r (l1 ++
-                     wn one :: map (fun _ : unit => wn (tens (wn one) bot)) (l7 ++ tt :: l2)))...
+                     wn one :: map (fun _ : unit => wn (tens (wn one) bot)) (l7 ++ tt :: l2)));
+          [ | cbn; Permutation_Type_solve ].
         apply IHl7.
-        eapply ex_r ; [ | apply Permutation_Type_app_comm ] ; list_simpl.
-        eapply ex_r ; [ | cons2app ; apply Permutation_Type_app_comm ] ; list_simpl.
+        eapply ex_r; [ | apply Permutation_Type_app_comm ] ; list_simpl.
+        eapply ex_r; [ | cons2app ; apply Permutation_Type_app_comm ] ; list_simpl.
         apply de_r.
-        eapply ex_r ; [ apply pi | ]... }
+        eapply ex_r; [ apply pi | ]; cbn; Permutation_Type_solve. }
       apply (Permutation_Type_app_head l1a) in HP3b.
       assert (IHP2 := Permutation_Type_trans HP1 HP3b).
       apply (@Permutation_Type_cons _ bot _ eq_refl) in IHP2.
       rewrite app_comm_cons in IHP2.
       apply IHpi2 in IHP2.
       assert (Permutation_Type (l2a ++ l1a) l') as HP' by Permutation_Type_solve.
-      eapply ex_bbb_r ; [ apply mix2_bbb_r | apply HP' ]...
+      eapply ex_bbb_r; [ apply mix2_bbb_r | apply HP' ].
       -- rewrite <- app_nil_l.
-         eapply bot_rev_bbb...
+         eapply bot_rev_bbb; [ eassumption | reflexivity ].
       -- apply (stronger_pfrag (pmixupd_point_pfrag (pmixupd_point_pfrag pfrag_ll 0 true) 2 true)) ;
-           [ | eapply ll_to_mix02'''_axcut ]...
-         ++ nsplit 4...
-            ** intros a; split with a...
+           [ | eapply ll_to_mix02'''_axcut ]; try reflexivity.
+         ++ repeat split .
+            ** intros a; split with a; reflexivity.
             ** intro n.
-               repeat (destruct n; myeasy)...
-         ++ intros a ; destruct a.
-         ++ intros a ; destruct a.
-         ++ eapply ex_r in pi1' ; [  | apply Permutation_Type_app_comm ]...
+               repeat (destruct n; try reflexivity; try now constructor).
+         ++ intros a; destruct a.
+         ++ intros a; destruct a.
+         ++ eapply ex_r in pi1'; [ | apply Permutation_Type_app_comm ]; eassumption.
     * symmetry in Heq2; decomp_map_inf Heq2; inversion Heq2.
 - assert (HP' := HP).
   symmetry in HP'.
   apply Permutation_Type_vs_cons_inv in HP'.
-  destruct HP' as [[l'l l'r] Heq] ; cbn in Heq.
+  destruct HP' as [[l'l l'r] Heq]; cbn in Heq.
   rewrite Heq in HP.
   apply Permutation_Type_cons_app_inv in HP.
-  dichot_elt_app_inf_exec Heq ; subst.
+  dichot_elt_app_inf_exec Heq; subst.
   + rewrite app_assoc in HP.
     apply (@Permutation_Type_cons _ B _ eq_refl) in HP.
     apply (@Permutation_Type_cons _ A _ eq_refl) in HP.
     rewrite 2 app_comm_cons in HP.
     apply IHpi in HP.
-    eapply ex_bbb_r ; [ apply parr_bbb_r | ]...
-  + dichot_elt_app_inf_exec Heq1 ; subst.
+    eapply ex_bbb_r; [ apply parr_bbb_r; eassumption | apply Permutation_Type_cons_app; reflexivity ].
+  + dichot_elt_app_inf_exec Heq1; subst.
     * symmetry in Heq0; decomp_map_inf Heq0; inversion Heq0.
     * symmetry in Heq2; decomp_map_inf Heq2; inversion Heq2.
 - assert (HP' := HP).
   symmetry in HP'.
   apply Permutation_Type_vs_cons_inv in HP'.
-  destruct HP' as [[l'l l'r] Heq] ; cbn in Heq.
+  destruct HP' as [[l'l l'r] Heq]; cbn in Heq.
   rewrite Heq in HP.
   apply Permutation_Type_cons_app_inv in HP.
-  dichot_elt_app_inf_exec Heq ; subst.
-  + eapply ex_bbb_r ; [ apply top_bbb_r | apply Permutation_Type_middle ]...
-  + dichot_elt_app_inf_exec Heq1 ; subst.
+  dichot_elt_app_inf_exec Heq; subst.
+  + eapply ex_bbb_r; [ apply top_bbb_r | apply Permutation_Type_middle ].
+  + dichot_elt_app_inf_exec Heq1; subst.
     * symmetry in Heq0; decomp_map_inf Heq0; inversion Heq0.
     * symmetry in Heq2; decomp_map_inf Heq2; inversion Heq2.
 - assert (HP' := HP).
   symmetry in HP'.
   apply Permutation_Type_vs_cons_inv in HP'.
-  destruct HP' as [[l'l l'r] Heq] ; cbn in Heq.
+  destruct HP' as [[l'l l'r] Heq]; cbn in Heq.
   rewrite Heq in HP.
   apply Permutation_Type_cons_app_inv in HP.
-  dichot_elt_app_inf_exec Heq ; subst.
+  dichot_elt_app_inf_exec Heq; subst.
   + rewrite app_assoc in HP.
     apply (@Permutation_Type_cons _ A _ eq_refl) in HP.
     rewrite app_comm_cons in HP.
     apply IHpi in HP.
-    eapply ex_bbb_r ; [ apply plus_bbb_r1 | ]...
-  + dichot_elt_app_inf_exec Heq1 ; subst.
+    eapply ex_bbb_r; [ apply plus_bbb_r1; eassumption | apply Permutation_Type_cons_app; reflexivity ].
+  + dichot_elt_app_inf_exec Heq1; subst.
     * symmetry in Heq0; decomp_map_inf Heq0; inversion Heq0.
     * symmetry in Heq2; decomp_map_inf Heq2; inversion Heq2.
 - assert (HP' := HP).
   symmetry in HP'.
   apply Permutation_Type_vs_cons_inv in HP'.
-  destruct HP' as [[l'l l'r] Heq] ; cbn in Heq.
+  destruct HP' as [[l'l l'r] Heq]; cbn in Heq.
   rewrite Heq in HP.
   apply Permutation_Type_cons_app_inv in HP.
-  dichot_elt_app_inf_exec Heq ; subst.
+  dichot_elt_app_inf_exec Heq; subst.
   + rewrite app_assoc in HP.
     apply (@Permutation_Type_cons _ A _ eq_refl) in HP.
     rewrite app_comm_cons in HP.
     apply IHpi in HP.
-    eapply ex_bbb_r ; [ apply plus_bbb_r2 | ]...
-  + dichot_elt_app_inf_exec Heq1 ; subst.
+    eapply ex_bbb_r ; [ apply plus_bbb_r2; eassumption | apply Permutation_Type_cons_app; reflexivity ].
+  + dichot_elt_app_inf_exec Heq1; subst.
     * symmetry in Heq0; decomp_map_inf Heq0; inversion Heq0.
     * symmetry in Heq2; decomp_map_inf Heq2; inversion Heq2.
 - assert (HP' := HP).
   symmetry in HP'.
   apply Permutation_Type_vs_cons_inv in HP'.
-  destruct HP' as [[l'l l'r] Heq] ; cbn in Heq.
+  destruct HP' as [[l'l l'r] Heq]; cbn in Heq.
   rewrite Heq in HP.
   apply Permutation_Type_cons_app_inv in HP.
-  dichot_elt_app_inf_exec Heq ; subst.
+  dichot_elt_app_inf_exec Heq; subst.
   + rewrite app_assoc in HP.
     assert (HP2 := HP).
     apply (@Permutation_Type_cons _ A _ eq_refl) in HP.
@@ -425,174 +416,164 @@ intros l pi; induction pi using ll_nested_ind; intros l' l0' l1' HP.
     apply (@Permutation_Type_cons _ B _ eq_refl) in HP2.
     rewrite app_comm_cons in HP2.
     apply IHpi2 in HP2.
-    eapply ex_bbb_r ; [ apply with_bbb_r | apply Permutation_Type_middle ]...
-  + dichot_elt_app_inf_exec Heq1 ; subst.
+    eapply ex_bbb_r ; [ apply with_bbb_r | apply Permutation_Type_middle ]; assumption.
+  + dichot_elt_app_inf_exec Heq1; subst.
     * symmetry in Heq0; decomp_map_inf Heq0; inversion Heq0.
     * symmetry in Heq2; decomp_map_inf Heq2; inversion Heq2.
 - assert (HP' := HP).
   symmetry in HP'.
   apply Permutation_Type_vs_cons_inv in HP'.
-  destruct HP' as [[l'l l'r] Heq] ; cbn in Heq.
+  destruct HP' as [[l'l l'r] Heq]; cbn in Heq.
   rewrite Heq in HP.
   apply Permutation_Type_cons_app_inv in HP.
-  dichot_elt_app_inf_exec Heq ; subst.
+  dichot_elt_app_inf_exec Heq; subst.
   + symmetry in HP.
     apply Permutation_Type_map_inv in HP as [l' Heq HP].
-    symmetry in Heq; decomp_map_inf Heq; cbn in Heq1, Heq2, Heq3, Heq5; subst ; cbn in HP.
+    symmetry in Heq; decomp_map_inf Heq; cbn in Heq1, Heq2, Heq3, Heq5; subst; cbn in HP.
     apply (Permutation_Type_map wn) in HP.
     list_simpl in HP.
-    rewrite app_assoc in HP.
-    rewrite <- map_app in HP.
+    rewrite app_assoc, <- map_app in HP.
     apply (@Permutation_Type_cons _ A _ eq_refl) in HP.
-    rewrite app_comm_cons in HP.
-    rewrite Heq2, Heq5 in HP.
+    rewrite app_comm_cons, Heq2, Heq5 in HP.
     apply IHpi in HP.
-    eapply ex_bbb_r ; [ apply oc_bbb_r | ]...
-  + dichot_elt_app_inf_exec Heq1 ; subst.
+    eapply ex_bbb_r;
+      [ apply oc_bbb_r; eassumption | apply Permutation_Type_cons_app; list_simpl; reflexivity ].
+  + dichot_elt_app_inf_exec Heq1; subst.
     * symmetry in Heq0; decomp_map_inf Heq0; inversion Heq0.
     * symmetry in Heq2; decomp_map_inf Heq2; inversion Heq2.
 - assert (HP' := HP).
   symmetry in HP'.
   apply Permutation_Type_vs_cons_inv in HP'.
-  destruct HP' as [[l'l l'r] Heq] ; cbn in Heq.
+  destruct HP' as [[l'l l'r] Heq]; cbn in Heq.
   rewrite Heq in HP.
   apply Permutation_Type_cons_app_inv in HP.
-  dichot_elt_app_inf_exec Heq ; subst.
+  dichot_elt_app_inf_exec Heq; subst.
   + rewrite app_assoc in HP.
     apply (@Permutation_Type_cons _ A _ eq_refl) in HP.
     rewrite app_comm_cons in HP.
     apply IHpi in HP.
-    eapply ex_bbb_r ; [ apply de_bbb_r | ]...
+    eapply ex_bbb_r ; [ apply de_bbb_r; eassumption | apply Permutation_Type_cons_app; reflexivity ].
   + dichot_elt_app_inf_exec Heq1 ; subst.
     * symmetry in Heq0; decomp_map_inf Heq0; inversion Heq0.
     * symmetry in Heq2; decomp_map_inf Heq2; cbn in Heq1, Heq2, Heq3; subst; cbn in HP.
       inversion Heq2 ; subst.
-      list_simpl in HP ; rewrite <- map_app in HP.
+      list_simpl in HP; rewrite <- map_app in HP.
       apply (@Permutation_Type_cons _ (tens (wn one) bot) _ eq_refl) in HP.
       assert (Permutation_Type (tens (wn one) bot :: l)
                                (l' ++ map (fun _ : unit => tens (wn one) bot) (tt :: l1')
                                    ++ map (fun _ : unit => wn (tens (wn one) bot)) (l1 ++ l4)))
         as HP' by (etransitivity ; [ apply HP | ] ; Permutation_Type_solve). 
-      apply IHpi in HP'...
+      apply IHpi in HP'; assumption.
 - assert (HP' := HP).
   symmetry in HP'.
   apply Permutation_Type_vs_cons_inv in HP'.
-  destruct HP' as [[l'l l'r] Heq] ; cbn in Heq.
+  destruct HP' as [[l'l l'r] Heq]; cbn in Heq.
   rewrite Heq in HP.
   apply Permutation_Type_cons_app_inv in HP.
-  dichot_elt_app_inf_exec Heq ; subst.
+  dichot_elt_app_inf_exec Heq; subst.
   + rewrite app_assoc in HP.
     apply IHpi in HP.
-    eapply ex_bbb_r ; [ apply wk_bbb_r | ]...
-  + dichot_elt_app_inf_exec Heq1 ; subst.
+    eapply ex_bbb_r; [ apply wk_bbb_r; eassumption | apply Permutation_Type_cons_app; reflexivity ].
+  + dichot_elt_app_inf_exec Heq1; subst.
     * symmetry in Heq0; decomp_map_inf Heq0; inversion Heq0.
     * symmetry in Heq2; decomp_map_inf Heq2 ; cbn in Heq1, Heq2, Heq3; subst; cbn in HP.
       inversion Heq2 ; subst.
-      list_simpl in HP ; rewrite <- map_app in HP.
-      apply IHpi in HP...
+      list_simpl in HP; rewrite <- map_app in HP.
+      apply IHpi in HP; assumption.
 - assert (HP' := HP).
   symmetry in HP'.
   apply Permutation_Type_vs_cons_inv in HP'.
-  destruct HP' as [[l'l l'r] Heq] ; cbn in Heq.
+  destruct HP' as [[l'l l'r] Heq]; cbn in Heq.
   rewrite Heq in HP.
   apply Permutation_Type_cons_app_inv in HP.
-  dichot_elt_app_inf_exec Heq ; subst.
+  dichot_elt_app_inf_exec Heq; subst.
   + rewrite app_assoc in HP.
     apply (@Permutation_Type_cons _ (wn A) _ eq_refl) in HP.
     apply (@Permutation_Type_cons _ (wn A) _ eq_refl) in HP.
     rewrite 2 app_comm_cons in HP.
     apply IHpi in HP.
-    eapply ex_bbb_r ; [ apply co_bbb_r | ]...
-  + dichot_elt_app_inf_exec Heq1 ; subst.
+    eapply ex_bbb_r; [ apply co_bbb_r; eassumption | apply Permutation_Type_cons_app; reflexivity ].
+  + dichot_elt_app_inf_exec Heq1; subst.
     * symmetry in Heq0; decomp_map_inf Heq0; inversion Heq0.
-    * symmetry in Heq2; decomp_map_inf Heq2 ; cbn in Heq1, Heq2, Heq3; subst; cbn in HP.
-      inversion Heq2 ; subst.
-      list_simpl in HP ; rewrite <- map_app in HP.
-    apply (@Permutation_Type_cons _ (wn (tens (wn one) bot)) _ eq_refl) in HP.
-    apply (@Permutation_Type_cons _ (wn (tens (wn one) bot)) _ eq_refl) in HP.
-    apply (@Permutation_Type_trans _ (wn (tens (wn one) bot) ::
-                                      wn (tens (wn one) bot) :: l)) in HP...
-    assert (Permutation_Type (wn (tens (wn one) bot) :: wn (tens (wn one) bot) :: l)
-       (l' ++ map (fun _ : unit => tens (wn one) bot) l1' ++
-              map (fun _ : unit => wn (tens (wn one) bot)) (tt :: tt :: l1 ++ l4)))
-      as HP' by (etransitivity ; [ apply HP | Permutation_Type_solve ]).
-    apply IHpi in HP'...
+    * symmetry in Heq2; decomp_map_inf Heq2; cbn in Heq1, Heq2, Heq3; subst; cbn in HP.
+      inversion Heq2; subst.
+      list_simpl in HP; rewrite <- map_app in HP.
+      apply (@Permutation_Type_cons _ (wn (tens (wn one) bot)) _ eq_refl) in HP.
+      apply (@Permutation_Type_cons _ (wn (tens (wn one) bot)) _ eq_refl) in HP.
+      apply (@Permutation_Type_trans _ (wn (tens (wn one) bot) ::
+                                        wn (tens (wn one) bot) :: l)) in HP; [ | reflexivity ].
+      assert (Permutation_Type (wn (tens (wn one) bot) :: wn (tens (wn one) bot) :: l)
+         (l' ++ map (fun _ : unit => tens (wn one) bot) l1' ++
+                map (fun _ : unit => wn (tens (wn one) bot)) (tt :: tt :: l1 ++ l4)))
+        as HP' by (etransitivity ; [ apply HP | Permutation_Type_solve ]).
+      apply IHpi in HP'; assumption.
 - inversion f.
 - destruct a.
 Qed.
 
 (** ** Cut admissibility for [ll_bbb] *)
 
-Theorem cut_bbb_r : forall A l1 l2,
-  ll_bbb (dual A :: l1) -> ll_bbb (A :: l2) -> ll_bbb (l2 ++ l1).
+Theorem cut_bbb_r A l1 l2 : ll_bbb (dual A :: l1) -> ll_bbb (A :: l2) -> ll_bbb (l2 ++ l1).
 Proof.
-intros A l1 l2 pi1 pi2.
+intros pi1 pi2.
 apply bbb_to_ll in pi1.
 apply bbb_to_ll in pi2.
-eapply ex_r in pi1 ; [ | apply Permutation_Type_swap ].
-eapply ex_r in pi2 ; [ | apply Permutation_Type_swap ].
+eapply ex_r in pi1; [ | apply Permutation_Type_swap ].
+eapply ex_r in pi2; [ | apply Permutation_Type_swap ].
 apply (cut_ll_r _ _ _ pi1) in pi2.
 apply (ex_r _ ((l2 ++ l1) ++ map (fun _ => tens (wn one) bot) (@nil unit)
-                            ++ map (fun _ => wn (tens (wn one) bot)) (tt :: tt :: nil))) in pi2 ;
+                          ++ map (fun _ => wn (tens (wn one) bot)) (tt :: tt :: nil))) in pi2;
  [ | cbn; Permutation_Type_solve ].
-eapply ll_to_bbb in pi2 ; [ | reflexivity ].
-assumption.
+eapply ll_to_bbb in pi2 ; [ eassumption | reflexivity ].
 Qed.
 
 
 (** ** Comparison with LL + [bot = oc bot] *)
 
-Lemma mix2_bb_r : forall l1 l2, llR (oc bot) l1 -> llR (oc bot) l2 ->
-  llR (oc bot) (l2 ++ l1).
-Proof with myeeasy.
-intros l1 l2 pi1 pi2.
-eapply (cut_r one)...
-- apply bot_r...
+Lemma mix2_bb_r l1 l2 : llR (oc bot) l1 -> llR (oc bot) l2 -> llR (oc bot) (l2 ++ l1).
+Proof.
+intros pi1 pi2.
+assert (pcut (pfrag_llR (oc bot : formula)) = true) as Hcut by reflexivity.
+apply (@cut_r _ _ Hcut one).
+- apply bot_r; assumption.
 - cons2app.
-  eapply (cut_r (oc bot)).
-  + apply wk_r...
+  apply (@cut_r _ _ Hcut (oc bot)).
+  + apply wk_r; assumption.
   + apply (@gax_r _ (pfrag_llR (oc bot)) false).
-Unshelve. all : reflexivity.
 Qed.
 
-Lemma mix2_to_bb : forall l, ll_mix2 l -> llR (oc bot) l.
-Proof with myeeasy.
-intros l pi; induction pi using ll_nested_ind ; try now econstructor.
-- eapply ex_r...
-- eapply ex_wn_r...
-- repeat (destruct L; try now inversion eqpmix).
-  cbn; rewrite app_nil_r.
-  apply mix2_bb_r...
-  + assert (In_inf l0 (l :: l0 :: nil)) as Hin.
-    { right; left... }
-    apply (In_Forall_inf_in _ PL) in Hin as [pi Hin].
-    refine (Dependent_Forall_inf_forall_formula _ _ X Hin).
-  + assert (In_inf l (l :: l0 :: nil)) as Hin by now left.
-    apply (In_Forall_inf_in _ PL) in Hin as [pi Hin].
-    refine (Dependent_Forall_inf_forall_formula _ _ X Hin).
+Lemma mix2_to_bb l : ll_mix2 l -> llR (oc bot) l.
+Proof.
+intros pi; induction pi using ll_nested_ind;
+  try (now constructor); try (econstructor; eassumption); try now econstructor.
+repeat (destruct L; try now inversion eqpmix).
+cbn; rewrite app_nil_r.
+apply mix2_bb_r.
+- assert (In_inf l0 (l :: l0 :: nil)) as Hin by (right; left; reflexivity).
+  apply (In_Forall_inf_in _ PL) in Hin as [pi Hin].
+  apply (Dependent_Forall_inf_forall_formula _ _ X Hin).
+- assert (In_inf l (l :: l0 :: nil)) as Hin by now left.
+  apply (In_Forall_inf_in _ PL) in Hin as [pi Hin].
+  apply (Dependent_Forall_inf_forall_formula _ _ X Hin).
 Qed.
 
-Theorem bb_to_bbb : forall l, llR (oc bot) l -> ll_bbb l.
-Proof with myeeasy ; try (cbn; Permutation_Type_solve).
-intros l pi.
-induction pi ; try now econstructor.
-- eapply ex_bbb_r...
-- eapply ex_bbb_r...
-  apply (Permutation_Type_map wn) in p ; Permutation_Type_solve.
-- eapply cut_bbb_r...
-- destruct a ; cbn.
-  + apply de_bbb_r.
-    apply one_bbb_r.
-  + rewrite <- (app_nil_l (one :: _)).
-    rewrite app_comm_cons.
+Theorem bb_to_bbb l : llR (oc bot) l -> ll_bbb l.
+Proof.
+intros pi; induction pi; try (now constructor).
+- econstructor; eassumption.
+- eapply ex_bbb_r; [ eassumption | ].
+  apply (Permutation_Type_map wn) in p; Permutation_Type_solve.
+- now econstructor.
+- eapply cut_bbb_r; eassumption.
+- destruct a; cbn.
+  + apply de_bbb_r, one_bbb_r.
+  + rewrite <- (app_nil_l (one :: _)), app_comm_cons.
     apply mix2_bbb_r.
     * apply one_bbb_r.
     * change nil with (map (@wn atom) nil).
-      apply oc_r.
-      eapply bot_r.
+      apply oc_r, bot_r.
       change (map wn nil) with (concat (@nil (list formula))).
-      apply mix_r...
-      apply Forall_inf_nil.
+      apply mix_r; constructor.
 Qed.
 
 (** The converse of [bb_to_bbb] is proved in the [nn] library. *)
@@ -600,74 +581,70 @@ Qed.
 (** *** Examples *)
 (*
 Goal ll_bbb (one :: oc (parr one one) :: nil).
-Proof with myeeasy.
+Proof.
 change (one :: oc (parr one one) :: nil)
-  with ((one :: nil) ++ oc (parr one one) :: nil).
-eapply mix2_bbb_r.
-- change nil with (map wn nil).
-  apply oc_bbb_r.
-  apply parr_bbb_r.
+  with ((one :: nil) ++ oc (parr one one) :: nil : list formula).
+apply mix2_bbb_r.
+- change nil with (map wn nil : list formula).
+  apply oc_bbb_r, parr_bbb_r.
   cbn.
-  change (one :: one :: nil) with ((one :: nil) ++ one :: nil).
+  change (one :: one :: nil) with ((one :: nil) ++ one :: nil : list formula).
   apply mix2_bbb_r.
   + apply one_bbb_r.
-  + eapply one_r.
-- eapply one_r.
+  + apply one_r.
+- apply one_r.
 Qed.
 
 Goal llR (oc bot) (one :: oc (parr one one) :: nil).
-Proof with myeeasy.
+Proof.
 assert (llR (oc bot) ((one :: nil) ++ one :: nil))
-  as Hr by (eapply mix2_bb_r ; apply one_r).
+  as Hr by (eapply mix2_bb_r; apply one_r).
 change (one :: oc (parr one one) :: nil)
-  with ((one :: nil) ++ oc (parr one one) :: nil).
-eapply mix2_bb_r.
-- change nil with (map wn nil).
-  apply oc_r.
-  apply parr_r...
+  with ((one :: nil) ++ oc (parr one one) :: nil : list formula).
+apply mix2_bb_r.
+- change nil with (map wn nil : list formula).
+  apply oc_r, parr_r; assumption.
 - apply one_r.
 Qed.
 *)
 
-Example bbb_ex :
-  ll_bbb (one :: oc (tens (parr one one) bot) :: nil).
-Proof with myeeasy ; try Permutation_Type_solve.
+Example bbb_ex : ll_bbb (one :: oc (tens (parr one one) bot) :: nil).
+Proof.
 change (one :: oc (tens (parr one one) bot) :: nil)
   with ((@one atom :: nil) ++ (oc (tens (parr one one) bot) :: nil)).
-apply (ex_bbb_r ((oc (tens (parr one one) bot) :: nil) ++ one :: nil))...
-eapply mix2_bbb_r.
+apply (@ex_bbb_r ((oc (tens (parr one one) bot) :: nil) ++ one :: nil));
+  [ | Permutation_Type_solve ].
+apply mix2_bbb_r.
 - apply one_bbb_r.
 - change (oc (tens (parr one one) bot) :: nil)
     with (@oc atom (tens (parr one one) bot) :: map wn (nil ++ nil)).
-  eapply oc_r.
+  apply oc_r.
   rewrite map_app.
-  eapply tens_r.
-  + eapply parr_r.
+  apply tens_r.
+  + apply parr_r.
     cbn.
     change (one :: one :: nil) with (concat ((@one atom :: nil) :: (one :: nil) :: nil)).
-    apply mix_r...
+    apply mix_r; [ reflexivity | ].
     repeat (apply Forall_inf_cons; try apply one_r).
     apply Forall_inf_nil.
-  + eapply bot_r.
+  + apply bot_r.
     change (map wn nil) with (concat (@nil (list formula))).
-    apply mix_r...
-    apply Forall_inf_nil.
+    apply mix_r; constructor.
 Qed.
 
-Example bb_ex :
-  llR (oc bot) (one :: oc (tens (parr one one) bot) :: nil).
-Proof with myeeasy.
+Example bb_ex : llR (oc bot) (one :: oc (tens (parr one one) bot) :: nil).
+Proof.
 assert (Hax := @gax_r _ (@pfrag_llR atom (oc bot)) false); cbn in Hax.
 assert (llR (oc bot) ((one :: nil) ++ one :: nil))
   as Hr by (eapply mix2_bb_r ; apply one_r).
-eapply (@cut_r _ (pfrag_llR _) eq_refl) in Hax...
+eapply (@cut_r _ (pfrag_llR _) eq_refl) in Hax.
 - apply Hax.
-- eapply ex_r ; [ | apply Permutation_Type_swap ].
+- eapply ex_r; [ | apply Permutation_Type_swap ].
   cbn; change (wn one :: nil) with (map (@wn atom) (one :: nil)).
   apply oc_r.
   cbn; rewrite <- (app_nil_l nil), app_comm_cons.
   apply tens_r.
-  + apply parr_r...
+  + apply parr_r; assumption.
   + apply bot_r, de_r, one_r.
 Qed.
 
@@ -696,137 +673,120 @@ Inductive ll_bbb0 : list formula -> Type :=
 (** The example given above in [ll_bbb] and [llR (oc bot)] is not cut-free provable
     in [ll_bbb0]. *)
 Lemma mix0_bbb0_false : ll_bbb0 nil -> False.
-Proof with myeasy.
+Proof.
 intros pi.
 remember nil as l.
-revert Heql ; induction pi ; intros Heql ; inversion Heql ; subst.
+revert Heql; induction pi; intros Heql; inversion Heql; subst.
 - symmetry in p.
-  apply Permutation_Type_nil in p ; intuition.
+  apply Permutation_Type_nil in p; auto.
 - apply app_eq_nil in Heql.
-  destruct Heql ; subst ; intuition.
+  destruct Heql; subst; auto.
 Qed.
 
-Lemma ex_implies_mix2_mix02 : forall l,
+Lemma ex_implies_mix2_mix02 l :
   ll_bbb0 l -> Permutation_Type l (one :: oc (tens (parr one one) bot) :: nil) ->
     @ll_mix0 atom (one :: one :: nil).
-Proof with myeeasy.
-intros l H; induction H; intro HP;
+Proof.
+intros pi; induction pi; intro HP;
   try now (apply Permutation_Type_sym in HP ;
-       apply Permutation_Type_length_2_inv in HP as [HP | HP] ;
-       inversion HP).
-- apply IHll_bbb0.
+           apply Permutation_Type_length_2_inv in HP as [HP | HP] ;
+           inversion HP).
+- apply IHpi.
   Permutation_Type_solve.
 - apply Permutation_Type_sym in HP.
-  apply Permutation_Type_length_2_inv in HP.
-  destruct HP as [HP | HP].
+  apply Permutation_Type_length_2_inv in HP as [HP | HP].
   + symmetry in HP.
     rewrite <- (app_nil_l (one :: _)) in HP.
-    dichot_elt_app_inf_exec HP ; subst.
+    dichot_elt_app_inf_exec HP; subst.
     * apply eq_sym in HP1.
       apply app_eq_unit_inf in HP1.
-      destruct HP1 ; destruct p ; subst.
-      -- clear - H.
+      destruct HP1; destruct p; subst.
+      -- clear - pi.
          exfalso.
          remember (oc (tens (parr one one) bot) :: nil) as l.
-         revert Heql ; induction H ; intro Heql ; inversion Heql ; subst.
+         revert Heql; induction pi; intro Heql; inversion Heql; subst.
          ++ symmetry in p.
             apply Permutation_Type_length_1_inv in p.
-            apply IHll_bbb0...
-         ++ apply app_eq_unit in Heql.
-            destruct Heql ; destruct H0 ; subst.
-            ** apply IHll_bbb0...
-            ** eapply mix0_bbb0_false...
-         ++ rewrite_all H2.
-            clear - H.
+            apply IHpi; assumption.
+         ++ apply app_eq_unit in Heql as [[-> ->] | [-> ->]].
+            ** apply IHpi; reflexivity.
+            ** apply mix0_bbb0_false; assumption.
+         ++ rewrite_all H1.
+            clear - pi.
             remember (tens (parr one one) bot :: nil) as l.
-            revert Heql ; induction H ; intro Heql ; inversion Heql ; subst.
+            revert Heql; induction pi; intro Heql; inversion Heql; subst.
             ** symmetry in p.
                apply Permutation_Type_length_1_inv in p.
-               apply IHll_bbb0...
-            ** apply app_eq_unit in Heql.
-               destruct Heql ; destruct H0 ; subst.
-               --- apply IHll_bbb0...
-               --- eapply mix0_bbb0_false...
-            ** apply app_eq_nil in H4.
-               destruct H4 ; subst.
-               clear - H0.
+               apply IHpi; assumption.
+            ** apply app_eq_unit in Heql as [[-> ->] | [-> ->]].
+               --- apply IHpi; reflexivity.
+               --- apply mix0_bbb0_false; assumption.
+            ** apply app_eq_nil in H2 as [-> ->].
+               clear - pi2.
                remember (bot :: nil) as l.
-               revert Heql ; induction H0 ; intro Heql ; inversion Heql ; subst.
+               revert Heql; induction pi2; intro Heql; inversion Heql; subst.
                --- symmetry in p.
-                   apply Permutation_Type_length_1_inv in p.
-                   apply IHll_bbb0...
-               --- apply app_eq_unit_inf in Heql.
-                   destruct Heql ; destruct p ; subst.
-                   +++ apply IHll_bbb0...
-                   +++ eapply mix0_bbb0_false...
-               --- eapply mix0_bbb0_false...
+                   apply Permutation_Type_length_1_inv in p as ->.
+                   apply IHpi2; reflexivity.
+               --- apply app_eq_unit in Heql as [[-> ->] | [-> ->]].
+                   +++ apply IHpi2; reflexivity.
+                   +++ apply mix0_bbb0_false; assumption.
+               --- apply mix0_bbb0_false; assumption.
       -- exfalso.
-         eapply mix0_bbb0_false...
+         apply mix0_bbb0_false; assumption.
     * symmetry in HP0.
       apply app_eq_nil in HP0.
-      destruct HP0 ; subst.
-      apply IHll_bbb0...
+      destruct HP0; subst.
+      apply IHpi; reflexivity.
   + symmetry in HP.
     rewrite <- (app_nil_l (oc _::_)) in HP.
-    dichot_elt_app_inf_exec HP ; subst.
+    dichot_elt_app_inf_exec HP; subst.
     * symmetry in HP1.
-      apply app_eq_unit_inf in HP1.
-      destruct HP1 ; destruct p ; subst.
-      -- clear - l ; rename l into H.
-         cbn in H.
+      apply app_eq_unit_inf in HP1 as [[-> ->] | [-> ->]].
+      -- clear - l ; rename l into pi; cbn in pi.
          remember (oc (tens (parr one one) bot) :: nil) as l.
-         revert Heql ; induction H ; intro Heql ; inversion Heql ; subst.
-         ++ symmetry in p.
-            cbn in p.
-            apply Permutation_Type_length_1_inv in p.
-            apply IHll...
-         ++ destruct l1 ; inversion Heql.
-            ** destruct lw' ; inversion Heql ; cbn in H0 ; subst.
-               symmetry in p ; apply Permutation_Type_nil in p ; subst.
-               intuition.
-            ** apply app_eq_nil in H3 ; destruct H3 as [Heq1 Heq2] ; subst.
-               apply app_eq_nil in Heq2 ; destruct Heq2 as [Heq2 ?] ; subst.
-               destruct lw' ; inversion Heq2 ; subst.
-               symmetry in p ; apply Permutation_Type_nil in p ; subst.
-               intuition.
+         revert Heql; induction pi; intro Heql; inversion Heql; subst.
+         ++ symmetry in p; cbn in p.
+            apply Permutation_Type_length_1_inv in p as ->.
+            apply IHpi; reflexivity.
+         ++ destruct l1; inversion Heql.
+            ** destruct lw'; inversion Heql; cbn in H; subst.
+               symmetry in p; apply Permutation_Type_nil in p as ->; auto.
+            ** apply app_eq_nil in H2 as [-> Heq2].
+               apply app_eq_nil in Heq2 as [Heq2 ->].
+               destruct lw'; inversion Heq2; subst.
+               symmetry in p; apply Permutation_Type_nil in p as ->; auto.
          ++ repeat (destruct L; inversion i; try now inversion Heql).
-         ++ rewrite_all H2.
-            clear - H.
+         ++ rewrite_all H1; clear - pi.
             remember (tens (parr one one) bot :: nil) as l.
-            revert Heql ; induction H ; intro Heql ; inversion Heql ; subst.
-            ** symmetry in p.
-               cbn in p.
-               apply Permutation_Type_length_1_inv in p.
-               apply IHll...
-            ** destruct l1 ; inversion Heql.
-               --- destruct lw' ; inversion Heql ; cbn in H0 ; subst.
-                   symmetry in p ; apply Permutation_Type_nil in p ; subst.
-                   intuition.
-               --- apply app_eq_nil in H3 ; destruct H3 as [Heq1 Heq2] ; subst.
-                   apply app_eq_nil in Heq2 ; destruct Heq2 as [Heq2 ?] ; subst.
-                   destruct lw' ; inversion Heq2 ; subst.
-                   symmetry in p ; apply Permutation_Type_nil in p ; subst.
-                   intuition.
+            revert Heql; induction pi; intro Heql; inversion Heql; subst.
+            ** symmetry in p; cbn in p.
+               apply Permutation_Type_length_1_inv in p as ->.
+               apply IHpi; reflexivity.
+            ** destruct l1; inversion Heql.
+               --- destruct lw'; inversion Heql; subst.
+                   symmetry in p; apply Permutation_Type_nil in p as ->; auto.
+               --- apply app_eq_nil in H2 as [-> Heq2].
+                   apply app_eq_nil in Heq2 as [Heq2 ->].
+                   destruct lw'; inversion Heq2; subst.
+                   symmetry in p; apply Permutation_Type_nil in p as ->; auto.
             ** repeat (destruct L; inversion i; try now inversion H0).
-            ** apply app_eq_nil in H4.
-               destruct H4 ; subst.
-               clear - H.
+            ** apply app_eq_nil in H2 as [-> ->].
+               clear - pi1.
                remember (parr one one :: nil) as l.
-               revert Heql ; induction H ; intro Heql ; inversion Heql ; subst...
-               --- symmetry in p.
-                   cbn in p.
-                   apply Permutation_Type_length_1_inv in p.
-                   apply IHll...
-               --- destruct l1 ; inversion Heql.
-                   +++ destruct lw' ; inversion Heql ; cbn in H0 ; subst.
-                       symmetry in p ; apply Permutation_Type_nil in p ; subst.
-                       intuition.
-                   +++ apply app_eq_nil in H3 ; destruct H3 as [Heq1 Heq2] ; subst.
-                       apply app_eq_nil in Heq2 ; destruct Heq2 as [Heq2 ?] ; subst.
-                       destruct lw' ; inversion Heq2 ; subst.
-                       symmetry in p ; apply Permutation_Type_nil in p ; subst.
-                       intuition.
+               revert Heql; induction pi1; intro Heql; inversion Heql; subst.
+               --- symmetry in p; cbn in p.
+                   apply Permutation_Type_length_1_inv in p as ->.
+                   apply IHpi1; reflexivity.
+               --- destruct l1; inversion Heql.
+                   +++ destruct lw'; inversion Heql; subst.
+                       symmetry in p; apply Permutation_Type_nil in p as ->; auto.
+                   +++ apply app_eq_nil in H2 as [-> Heq2].
+                       apply app_eq_nil in Heq2 as [Heq2 ->].
+                       destruct lw'; inversion Heq2; subst.
+                       symmetry in p; apply Permutation_Type_nil in p as ->; auto.
                --- repeat (destruct L; inversion i; try now inversion H0).
+               --- assumption.
                --- inversion f.
                --- destruct a.
             ** inversion f.
@@ -834,69 +794,54 @@ intros l H; induction H; intro HP;
          ++ inversion f.
          ++ destruct a.
       -- exfalso.
-         eapply mix0_bbb0_false...
+         apply mix0_bbb0_false; assumption.
     * symmetry in HP0.
-      apply app_eq_nil in HP0.
-      destruct HP0 ; subst.
-      apply IHll_bbb0.
-      Permutation_Type_solve.
+      apply app_eq_nil in HP0 as [-> ->].
+      apply IHpi, Permutation_Type_swap.
 - symmetry in HP.
-  apply Permutation_Type_length_2_inv in HP.
-  destruct HP as [HP | HP] ; inversion HP.
-  destruct l ; inversion H2.
-Defined.
+  apply Permutation_Type_length_2_inv in HP as [HP | HP] ; inversion HP.
+  destruct l; inversion H1.
+Qed.
 
 Lemma ex_not_bbb0 :
   ll_bbb0 (one :: oc (tens (parr one one) bot) :: nil) -> False.
 Proof.
-intros H.
+intros pi.
 apply (@mix0_not_mix2 atom).
 eapply ex_implies_mix2_mix02 ; [ eassumption | reflexivity ].
 Qed.
 
 Lemma bbb_neq_bbb0 : { l & prod (ll_bbb l) (ll_bbb0 l -> False) }.
-Proof.
-eexists ; split ; [ apply bbb_ex | apply ex_not_bbb0 ].
-Qed.
+Proof. eexists; split; [ apply bbb_ex | apply ex_not_bbb0 ]. Qed.
 
 (** The same example is provable in [ll_bbb0] with cut,
     thus cut admissibility does not hold for [ll_bbb0]. *)
 
 Section bbb0_with_cut.
 
-Hypothesis cut_bbb0_r : forall A l1 l2,
+Variable cut_bbb0_r : forall A l1 l2,
   ll_bbb0 (dual A :: l1) -> ll_bbb0 (A :: l2) -> ll_bbb0 (l2 ++ l1).
 
-Theorem llR_oc_bot_to_bbb0_cut : forall l,
-  llR (oc bot) l -> ll_bbb0 l.
-Proof with myeeasy.
-intros l pi.
-induction pi ; (try now inversion f) ; try now constructor.
-- eapply ex_bbb0_r...
-- eapply ex_bbb0_r...
-  apply (Permutation_Type_map wn) in p ; Permutation_Type_solve.
-- eapply cut_bbb0_r...
-- destruct a ; cbn.
-  + apply de_bbb0_r.
-    apply one_bbb0_r.
-  + rewrite <- (app_nil_l (one :: _)).
-    rewrite app_comm_cons.
+Theorem llR_oc_bot_to_bbb0_cut l : llR (oc bot) l -> ll_bbb0 l.
+Proof.
+intros pi; induction pi; (try now inversion f); try now constructor.
+- eapply ex_bbb0_r; eassumption.
+- eapply ex_bbb0_r; [ eassumption | ].
+  apply (Permutation_Type_map wn) in p; Permutation_Type_solve.
+- eapply cut_bbb0_r; eassumption.
+- destruct a; cbn.
+  + apply de_bbb0_r, one_bbb0_r.
+  + rewrite <- (app_nil_l (one :: _)), app_comm_cons.
     apply mix2_bbb0_r.
     * apply one_bbb0_r.
     * change nil with (map (@wn atom) nil).
-      apply oc_r.
-      eapply bot_r.
+      apply oc_r, bot_r.
       change (map wn nil) with (concat (@nil (list formula))).
-      apply mix_r...
-      apply Forall_inf_nil.
+      apply mix_r; constructor.
 Qed.
 
-Example bbb0_cut_ex :
-  ll_bbb0 (one :: oc (tens (parr one one) bot) :: nil).
-Proof.
-apply llR_oc_bot_to_bbb0_cut.
-apply bb_ex.
-Qed.
+Example bbb0_cut_ex : ll_bbb0 (one :: oc (tens (parr one one) bot) :: nil).
+Proof. apply llR_oc_bot_to_bbb0_cut, bb_ex. Qed.
 
 End bbb0_with_cut.
 
@@ -904,11 +849,6 @@ Lemma cut_not_rule_bbb0 :
 (forall A l1 l2,
   ll_bbb0 (dual A :: l1) -> ll_bbb0 (A :: l2) -> ll_bbb0 (l2 ++ l1))
     -> False.
-Proof.
-intros Hcut.
-apply ex_not_bbb0.
-apply bbb0_cut_ex.
-assumption.
-Qed.
+Proof. intros Hcut; apply ex_not_bbb0, bbb0_cut_ex, Hcut. Qed.
 
 End Atoms.
